src/Noninterference/LoggedDisk/ATCD_Commit_Pre.v
@@ -1,0 +1,635 @@
+Require Import Eqdep Lia Lra Framework FSParameters FileDiskLayer. (* LoggedDiskLayer TransactionCacheLayer TransactionalDiskLayer. *)
+Require Import FileDiskNoninterference LoggedDiskRefinement.
+Require Import ATC_ORS HSS ATCDLayer ATCD_Simulation ATCD_AOE.
+Require Import LogCache_FinishedNotCrashed ATCD_ORS ATCD_HSS.
+Import FileDiskLayer.
+
+Lemma disk_allocator_read_exact_txn:
+  forall u o s1 s1' r v1,
+exec ATCLang u o s1
+  (RefinementLift.compile
+     (HorizontalComposition AuthenticationOperation
+        TransactionCacheOperation)
+     (HorizontalComposition AuthenticationOperation
+        (TransactionalDiskLayer.TDCore data_length)) ATCLang AD
+     (HC_Core_Refinement ATCLang AD Definitions.TDCoreRefinement)
+     (option _)
+     (@lift_L2 AuthenticationOperation _ TD _ (File.DiskAllocator.read v1)))
+  (Finished s1' r) ->
+     s1' = s1.
+     Proof.
+      Transparent File.DiskAllocator.read.
+      unfold File.DiskAllocator.read.
+      intros; cleanup; simpl in *; repeat invert_exec;
+      simpl in *; repeat invert_exec; eauto;
+      eapply Transaction.read_finished_state in H2; eauto;
+      cleanup; eauto; repeat cleanup_pairs;
+      try eapply Transaction.read_finished_state in H3; eauto;
+      cleanup; eauto.
+    destruct s1'; eauto.
+      Opaque File.DiskAllocator.read.
+    Qed.
+
+Lemma inode_allocator_write_exact_txn:
+    forall u o s1 s1' r inum v,
+  exec ATCLang u o s1
+    (RefinementLift.compile
+       (HorizontalComposition AuthenticationOperation
+          TransactionCacheOperation)
+       (HorizontalComposition AuthenticationOperation
+          (TransactionalDiskLayer.TDCore data_length)) ATCLang AD
+       (HC_Core_Refinement ATCLang AD Definitions.TDCoreRefinement)
+       (option _)
+       (@lift_L2 AuthenticationOperation _ TD _ (Inode.InodeAllocator.write inum v)))
+    (Finished s1' (Some r)) ->
+    fst (snd s1') = (Inode.InodeAllocatorParams.bitmap_addr + S inum, v) :: fst (snd s1) /\
+    snd (snd s1') = snd (snd s1).
+       Proof.
+        Transparent Inode.InodeAllocator.write.
+        unfold Inode.InodeAllocator.write.
+        intros; cleanup; simpl in *; repeat invert_exec;
+        simpl in *; repeat invert_exec; eauto; try congruence.
+        eapply Transaction.read_finished_state in H2; eauto;
+        cleanup; eauto; repeat cleanup_pairs;
+        try eapply Transaction.write_finished_state in H4; eauto;
+        cleanup; eauto.
+        split_ors; cleanup; try congruence; eauto.
+        Opaque Inode.InodeAllocator.write.
+      Qed.
+
+Lemma disk_allocator_write_exact_txn:
+      forall u o s1 s1' r a v1,
+      exec ATCLang u o s1
+      (RefinementLift.compile
+          (HorizontalComposition AuthenticationOperation
+              TransactionCacheOperation)
+          (HorizontalComposition AuthenticationOperation
+              (TransactionalDiskLayer.TDCore data_length)) ATCLang AD
+          (HC_Core_Refinement ATCLang AD Definitions.TDCoreRefinement)
+          (option unit)
+          (@lift_L2 AuthenticationOperation _ TD _ (File.DiskAllocator.write a v1)))
+      (Finished s1' (Some r)) ->
+          fst (snd s1') = (File.DiskAllocatorParams.bitmap_addr + S a, v1) :: fst (snd s1) /\
+          snd (snd s1') = snd (snd s1) /\
+          a < File.DiskAllocatorParams.num_of_blocks.
+      Proof.
+          Transparent File.DiskAllocator.write.
+          unfold File.DiskAllocator.write.
+          intros; cleanup; simpl in *; repeat invert_exec;
+          simpl in *; repeat invert_exec; eauto; try congruence.
+          eapply Transaction.read_finished_state in H2; eauto;
+          cleanup; eauto; try congruence.
+          repeat cleanup_pairs;
+          eapply Transaction.write_finished_state in H4; eauto;
+          cleanup; eauto; try congruence.
+          repeat cleanup_pairs; eauto;
+          split_ors; cleanup; try lia.
+          simpl; intuition.
+      Qed.
+
+(***********)
+
+Lemma get_inode_exact_txn:
+forall u o s1 s1' r1 inum,
+exec ATCLang u o s1
+   (RefinementLift.compile
+      (HorizontalComposition AuthenticationOperation
+         TransactionCacheOperation)
+      (HorizontalComposition AuthenticationOperation
+         (TransactionalDiskLayer.TDCore data_length)) ATCLang AD
+      (HC_Core_Refinement ATCLang AD Definitions.TDCoreRefinement)
+      (option Inode.Inode)
+      (@lift_L2 AuthenticationOperation _ TD _ (Inode.get_inode inum)))
+   (Finished s1' r1) ->
+   s1 = s1'.
+   Proof.
+    Transparent Inode.get_inode.
+    unfold Inode.get_inode, Inode.InodeAllocator.read.
+    intros; cleanup; simpl in *; repeat invert_exec;
+    simpl in *; repeat invert_exec; eauto;
+    eapply Transaction.read_finished_state in H3; eauto;
+    cleanup; eauto;
+    repeat cleanup_pairs; eauto.
+    eapply Transaction.read_finished_state in H1; eauto;
+    cleanup; eauto.
+    destruct s1'; eauto.
+    Opaque Inode.get_inode.
+  Qed.
+
+Lemma inode_get_block_number_exact_txn:
+    forall u o s1 s1' r  inum a,
+    exec ATCLang u o s1
+    (RefinementLift.compile
+    (HorizontalComposition AuthenticationOperation
+    TransactionCacheOperation)
+    (HorizontalComposition AuthenticationOperation
+    (TransactionalDiskLayer.TDCore data_length)) ATCLang AD
+    (HC_Core_Refinement ATCLang AD Definitions.TDCoreRefinement)
+    (option _)
+    (@lift_L2 AuthenticationOperation _ TD _ (Inode.get_block_number inum a)))
+    (Finished s1' r) ->
+    s1'= s1.
+Proof.
+    Transparent Inode.get_block_number.
+    Opaque Inode.get_inode.
+    unfold Inode.get_block_number.
+    intros; cleanup; simpl in *; repeat invert_exec;
+    simpl in *; repeat invert_exec; eauto;
+    intros; cleanup; simpl in *; repeat invert_exec;
+    simpl in *; repeat invert_exec; eauto;
+    eapply get_inode_exact_txn in H; eauto; cleanup; eauto.
+    Opaque Inode.get_block_number.
+Qed.
+
+Lemma inode_get_all_block_numbers_exact_txn:
+    forall u o s1 s1' r  inum,
+    exec ATCLang u o s1
+    (RefinementLift.compile
+    (HorizontalComposition AuthenticationOperation
+    TransactionCacheOperation)
+    (HorizontalComposition AuthenticationOperation
+    (TransactionalDiskLayer.TDCore data_length)) ATCLang AD
+    (HC_Core_Refinement ATCLang AD Definitions.TDCoreRefinement)
+    (option _)
+    (@lift_L2 AuthenticationOperation _ TD _ (Inode.get_all_block_numbers inum)))
+    (Finished s1' r) ->
+    s1'= s1.
+Proof.
+    Transparent Inode.get_all_block_numbers.
+    Opaque Inode.get_inode.
+    unfold Inode.get_all_block_numbers.
+    intros; cleanup; simpl in *; repeat invert_exec;
+    simpl in *; repeat invert_exec; eauto;
+    intros; cleanup; simpl in *; repeat invert_exec;
+    simpl in *; repeat invert_exec; eauto;
+    eapply get_inode_exact_txn in H; eauto; cleanup; eauto.
+    Opaque Inode.get_all_block_numbers.
+Qed.
+
+Lemma inode_extend_exact_txn:
+    forall u o s1 s1' r inum a,
+    exec ATCLang u o s1
+    (RefinementLift.compile
+    (HorizontalComposition AuthenticationOperation
+    TransactionCacheOperation)
+    (HorizontalComposition AuthenticationOperation
+    (TransactionalDiskLayer.TDCore data_length)) ATCLang AD
+    (HC_Core_Refinement ATCLang AD Definitions.TDCoreRefinement)
+    (option _)
+    (@lift_L2 AuthenticationOperation _ TD _ (Inode.extend inum a)))
+    (Finished s1' (Some r)) ->
+    exists v,
+    fst (snd s1') = (Inode.InodeAllocatorParams.bitmap_addr + S inum, v) :: fst (snd s1) /\
+    snd (snd s1') = snd (snd s1).
+Proof.
+    Transparent Inode.extend.
+    unfold Inode.extend, Inode.set_inode.
+    intros; cleanup; simpl in *; repeat invert_exec;
+    simpl in *; repeat invert_exec; eauto;
+    intros; cleanup; simpl in *; repeat invert_exec;
+    simpl in *; repeat invert_exec; eauto; try congruence;
+    eapply get_inode_exact_txn in H; eauto; cleanup; eauto;
+    eapply inode_allocator_write_exact_txn in H0; eauto; cleanup; eauto.
+    Opaque Inode.extend.
+    Qed.
+
+Lemma inode_free_exact_txn:
+    forall u o s1 s1' r v1,
+exec ATCLang u o s1
+    (RefinementLift.compile
+       (HorizontalComposition AuthenticationOperation
+          TransactionCacheOperation)
+       (HorizontalComposition AuthenticationOperation
+          (TransactionalDiskLayer.TDCore data_length)) ATCLang AD
+       (HC_Core_Refinement ATCLang AD Definitions.TDCoreRefinement)
+       (option unit)
+       (@lift_L2 AuthenticationOperation _ TD _ (Inode.free v1)))
+    (Finished s1' (Some r)) ->
+       (exists new_bitmap, 
+       fst (snd s1') = (Inode.InodeAllocatorParams.bitmap_addr, new_bitmap) :: fst (snd s1) /\
+       snd (snd s1') = snd (snd s1)).
+       Proof.
+        Transparent Inode.free.
+        unfold Inode.free, Inode.InodeAllocator.free.
+        intros; cleanup; simpl in *; repeat invert_exec;
+        simpl in *; repeat invert_exec; eauto;
+        try eapply Transaction.read_finished_state in H2; eauto;
+        cleanup; eauto.
+          eapply Transaction.write_finished_state in H4; eauto;
+          cleanup; eauto;
+          repeat split_ors; cleanup; try congruence.
+          eexists; cleanup.
+          setoid_rewrite H4; simpl; eauto.
+          repeat cleanup_pairs; intuition eauto.
+        Qed.
+
+
+(***********)
+
+Lemma read_inner_exact_txn:
+forall u o s1 s1' r inum a,
+exec ATCLang u o s1
+(RefinementLift.compile
+(HorizontalComposition AuthenticationOperation
+TransactionCacheOperation)
+(HorizontalComposition AuthenticationOperation
+(TransactionalDiskLayer.TDCore data_length)) ATCLang AD
+(HC_Core_Refinement ATCLang AD Definitions.TDCoreRefinement)
+(option _)
+(@lift_L2 AuthenticationOperation _ TD _ (File.read_inner a inum)))
+(Finished s1' r) ->
+s1' = s1.
+Proof.
+unfold File.read_inner.
+intros; cleanup; simpl in *; repeat invert_exec;
+simpl in *; repeat invert_exec; eauto;
+intros; cleanup; simpl in *; repeat invert_exec;
+simpl in *; repeat invert_exec; eauto;
+eapply inode_get_block_number_exact_txn in H; eauto; cleanup; eauto;
+eapply disk_allocator_read_exact_txn in H0; eauto; cleanup; eauto.
+Qed.
+
+Lemma write_inner_commit_pre':
+forall u o s1 s1' r inum a v,
+exec ATCLang u o s1
+(RefinementLift.compile
+(HorizontalComposition AuthenticationOperation
+TransactionCacheOperation)
+(HorizontalComposition AuthenticationOperation
+(TransactionalDiskLayer.TDCore data_length)) ATCLang AD
+(HC_Core_Refinement ATCLang AD Definitions.TDCoreRefinement)
+(option _)
+(@lift_L2 AuthenticationOperation _ TD _ (File.write_inner a v inum)))
+(Finished s1' (Some r)) ->
+exists a, 
+fst (snd s1') = (File.DiskAllocatorParams.bitmap_addr + S a, v) :: fst (snd s1) /\
+snd (snd s1') = snd (snd s1) /\
+a < File.DiskAllocatorParams.num_of_blocks.
+Proof.
+unfold File.write_inner.
+intros; cleanup; simpl in *; repeat invert_exec;
+simpl in *; repeat invert_exec; eauto;
+intros; cleanup; simpl in *; repeat invert_exec;
+simpl in *; repeat invert_exec; eauto;
+eapply inode_get_block_number_exact_txn in H; eauto; cleanup; eauto;
+eapply disk_allocator_write_exact_txn in H0; eauto; cleanup; eauto;
+repeat cleanup_pairs; intuition eauto.
+Qed.
+
+Lemma change_owner_inner_exact_txn:
+forall u o s1 s1' r inum u',
+exec ATCLang u o s1
+(RefinementLift.compile
+(HorizontalComposition AuthenticationOperation
+TransactionCacheOperation)
+(HorizontalComposition AuthenticationOperation
+(TransactionalDiskLayer.TDCore data_length)) ATCLang AD
+(HC_Core_Refinement ATCLang AD Definitions.TDCoreRefinement)
+(option _)
+(@lift_L2 AuthenticationOperation _ TD _ (File.change_owner_inner u' inum)))
+(Finished s1' (Some r)) ->
+exists inode, 
+fst (snd s1') = (Inode.InodeAllocatorParams.bitmap_addr + S inum, inode) :: fst (snd s1) /\
+snd (snd s1') = snd (snd s1).
+Proof.
+Transparent Inode.change_owner.
+unfold File.change_owner_inner, Inode.change_owner, Inode.set_inode.
+intros; cleanup; simpl in *; repeat invert_exec;
+simpl in *; repeat invert_exec; eauto;
+intros; cleanup; simpl in *; repeat invert_exec;
+simpl in *; repeat invert_exec; eauto;
+eapply get_inode_exact_txn in H; eauto; cleanup; eauto;
+eapply inode_allocator_write_exact_txn in H0; eauto; cleanup; eauto;
+repeat cleanup_pairs; intuition eauto.
+Qed.
+
+Lemma extend_inner_commit_pre':
+forall u o s1 s1' r td1 inum v,
+Transaction.transaction_rep (snd s1) td1 ->
+exec ATCLang u o s1
+(RefinementLift.compile
+(HorizontalComposition AuthenticationOperation
+TransactionCacheOperation)
+(HorizontalComposition AuthenticationOperation
+(TransactionalDiskLayer.TDCore data_length)) ATCLang AD
+(HC_Core_Refinement ATCLang AD Definitions.TDCoreRefinement)
+(option _)
+(@lift_L2 AuthenticationOperation _ TD _ (File.extend_inner v inum)))
+(Finished s1' (Some r)) ->
+exists new_bitmap a i, 
+fst (snd s1') = (Inode.InodeAllocatorParams.bitmap_addr + S inum, i) :: (File.DiskAllocatorParams.bitmap_addr, new_bitmap) :: (File.DiskAllocatorParams.bitmap_addr + S a, v) :: fst (snd s1) /\
+snd (snd s1') = snd (snd s1) /\
+a < File.DiskAllocatorParams.num_of_blocks.
+Proof.
+Opaque File.DiskAllocator.alloc.
+unfold File.extend_inner.
+intros; cleanup; simpl in *; repeat invert_exec;
+simpl in *; repeat invert_exec; eauto;
+intros; cleanup; simpl in *; repeat invert_exec;
+simpl in *; repeat invert_exec; eauto;
+eapply disk_allocator_alloc_exact_txn in H0; eauto; cleanup; eauto;
+split_ors; cleanup; try congruence; repeat cleanup_pairs.
+eapply inode_extend_exact_txn in H1; simpl; eauto; cleanup; eauto;
+repeat cleanup_pairs; cleanup; intuition eauto; try congruence.
+do 3 eexists; intuition eauto.
+Qed.
+
+Lemma delete_inner_commit_pre':
+forall u o s1 s1' r td1 inum im,
+Transaction.transaction_rep (snd s1) td1 ->
+Inode.inode_rep im (fst (snd td1)) ->
+exec ATCLang u o s1
+(RefinementLift.compile
+(HorizontalComposition AuthenticationOperation
+TransactionCacheOperation)
+(HorizontalComposition AuthenticationOperation
+(TransactionalDiskLayer.TDCore data_length)) ATCLang AD
+(HC_Core_Refinement ATCLang AD Definitions.TDCoreRefinement)
+(option _)
+(@lift_L2 AuthenticationOperation _ TD _ (File.delete_inner inum)))
+(Finished s1' (Some r)) ->
+exists l i inode,
+im inum = Some inode /\
+fst (snd s1') = (Inode.InodeAllocatorParams.bitmap_addr, i) ::  l ++ fst (snd s1) /\
+(map fst l = repeat File.DiskAllocatorParams.bitmap_addr (length (Inode.block_numbers inode)))  /\
+snd (snd s1') = snd (snd s1).
+Proof.
+Opaque File.DiskAllocator.alloc.
+unfold File.delete_inner.
+intros; cleanup; simpl in *; repeat invert_exec;
+simpl in *; repeat invert_exec; eauto;
+intros; cleanup; simpl in *; repeat invert_exec;
+simpl in *; repeat invert_exec; eauto;
+eapply_fresh inode_get_all_block_numbers_exact_txn in H1; eauto; cleanup; eauto;
+cleanup; try congruence.
+
+eapply_fresh ATC_Simulation.ATC_oracle_refines_finished in H1; eauto.
+2: {
+    unfold HC_refines; simpl; eexists (_, _); intuition eauto.
+}
+cleanup.
+eapply_fresh ATC_Simulation.ATC_exec_lift_finished in H1; eauto;
+try solve [apply TransactionToTransactionalDisk.Refinement.TC_to_TD_core_simulation_finished];
+cleanup.
+2: {
+    simpl.
+    unfold HC_refines; simpl; instantiate (1:= (_, _)); intuition eauto.
+}
+
+eapply_fresh lift2_invert_exec in H5; cleanup_no_match.
+eapply Inode.get_all_block_numbers_finished in H9; eauto.
+cleanup; repeat split_ors; try congruence; cleanup.
+
+eapply free_all_blocks_exact_txn in H2; simpl; eauto; cleanup; eauto;
+repeat cleanup_pairs; cleanup; intuition eauto; try congruence.
+cleanup.
+eapply inode_free_exact_txn in H3; cleanup;
+repeat cleanup_pairs.
+repeat eexists; eauto.
+Unshelve.
+exact id.
+Qed.
+
+(*********)
+Lemma refines_related_txn_empty:
+    forall s1 s2 u ex,
+    refines_related ATC_Refinement (AD_related_states u ex) s1 s2 ->
+    (fst (snd s1)) = [] /\ (fst (snd s2)) = [].
+    Proof.
+    unfold AD_related_states, refines_related; simpl;
+    unfold HC_refines; simpl;
+    unfold TransactionToTransactionalDisk.Definitions.refines,
+    FileToFileDisk.Definitions.refines,
+    FD_related_states,
+    File.files_rep,
+    Transaction.transaction_rep; simpl.
+    intros; logic_clean; repeat split_ors; logic_clean; try congruence.
+    repeat cleanup_pairs.
+    destruct s, s3; simpl in *; try lia; eauto.
+    Qed.
+
+Theorem read_inner_commit_pre:
+forall u u' off inum (s0 s3 : state ATCLang) (o : oracle' ATCCore)
+  (s1' s2' : LayerImplementation.state' ATCCore) 
+  (r1 r2 : value),
+refines_related ATC_Refinement (AD_related_states u' None) s0 s3 ->
+exec ATCLang u o s0
+  (Simulation.Definitions.compile ATC_Refinement
+     (@lift_L2 AuthenticationOperation _ TD _ (File.read_inner off inum)))
+  (Finished s1' (Some r1)) ->
+exec ATCLang u o s3
+  (Simulation.Definitions.compile ATC_Refinement
+     (@lift_L2 AuthenticationOperation _ TD _ (File.read_inner off inum)))
+  (Finished s2' (Some r2)) ->
+length (dedup_last addr_dec (rev (map fst (fst (snd s1'))))) =
+length (dedup_last addr_dec (rev (map fst (fst (snd s2'))))) /\
+(Forall (fun a : nat => a < data_length)
+   (map fst (fst (snd s1'))) <->
+ Forall (fun a : nat => a < data_length)
+   (map fst (fst (snd s2')))).
+   Proof.
+    intros.
+    eapply read_inner_exact_txn in H0, H1; subst; eauto.
+    eapply refines_related_txn_empty in H; cleanup; 
+    simpl; intuition eauto.
+   Qed.
+
+   Theorem write_inner_commit_pre:
+   forall u u' ex off inum v1 v2 (s0 s3 : state ATCLang) (o : oracle' ATCCore)
+     (s1' s2' : LayerImplementation.state' ATCCore) 
+     r1 r2,
+   refines_related ATC_Refinement (AD_related_states u' ex) s0 s3 ->
+   exec ATCLang u o s0
+     (Simulation.Definitions.compile ATC_Refinement
+        (@lift_L2 AuthenticationOperation _ TD _ (File.write_inner off v1 inum)))
+     (Finished s1' (Some r1)) ->
+   exec ATCLang u o s3
+     (Simulation.Definitions.compile ATC_Refinement
+        (@lift_L2 AuthenticationOperation _ TD _ (File.write_inner off v2 inum)))
+     (Finished s2' (Some r2)) ->
+   length (dedup_last addr_dec (rev (map fst (fst (snd s1'))))) =
+   length (dedup_last addr_dec (rev (map fst (fst (snd s2'))))) /\
+   (Forall (fun a : nat => a < data_length)
+      (map fst (fst (snd s1'))) <->
+    Forall (fun a : nat => a < data_length)
+      (map fst (fst (snd s2')))).
+      Proof.
+       intros.
+       eapply write_inner_commit_pre' in H0, H1; subst; eauto.
+       cleanup; simpl.
+       eapply refines_related_txn_empty in H; cleanup; 
+       repeat cleanup_pairs; eauto.
+       pose proof file_blocks_fit_in_disk.
+       unfold File.DiskAllocatorParams.bitmap_addr,
+       File.DiskAllocatorParams.num_of_blocks in *.
+       simpl; intuition eauto;
+       repeat constructor; lia.
+    Qed.
+
+    Theorem change_owner_inner_commit_pre:
+   forall u u' ex inum v1 v2 (s0 s3 : state ATCLang) (o : oracle' ATCCore)
+     (s1' s2' : LayerImplementation.state' ATCCore) 
+     r1 r2,
+   refines_related ATC_Refinement (AD_related_states u' ex) s0 s3 ->
+   exec ATCLang u o s0
+     (Simulation.Definitions.compile ATC_Refinement
+        (@lift_L2 AuthenticationOperation _ TD _ (File.change_owner_inner v1 inum)))
+     (Finished s1' (Some r1)) ->
+   exec ATCLang u o s3
+     (Simulation.Definitions.compile ATC_Refinement
+        (@lift_L2 AuthenticationOperation _ TD _ (File.change_owner_inner v2 inum)))
+     (Finished s2' (Some r2)) ->
+   length (dedup_last addr_dec (rev (map fst (fst (snd s1'))))) =
+   length (dedup_last addr_dec (rev (map fst (fst (snd s2'))))) /\
+   (Forall (fun a : nat => a < data_length)
+      (map fst (fst (snd s1'))) <->
+    Forall (fun a : nat => a < data_length)
+      (map fst (fst (snd s2')))).
+      Proof.
+       intros.
+       eapply change_owner_inner_exact_txn in H0, H1; subst; eauto.
+       cleanup; simpl.
+       eapply refines_related_txn_empty in H; cleanup; 
+       repeat cleanup_pairs; eauto.
+       pose proof file_blocks_fit_in_disk.
+       unfold File.DiskAllocatorParams.bitmap_addr,
+       File.DiskAllocatorParams.num_of_blocks in *.
+       simpl; intuition eauto;
+       repeat constructor; lia.
+    Qed.
+
+    Theorem extend_inner_commit_pre:
+   forall u u' ex inum v1 v2 (s0 s3 : state ATCLang) (o : oracle' ATCCore)
+     (s1' s2' : LayerImplementation.state' ATCCore) 
+     r1 r2,
+   refines_related ATC_Refinement (AD_related_states u' ex) s0 s3 ->
+   exec ATCLang u o s0
+     (Simulation.Definitions.compile ATC_Refinement
+        (@lift_L2 AuthenticationOperation _ TD _ (File.extend_inner v1 inum)))
+     (Finished s1' (Some r1)) ->
+   exec ATCLang u o s3
+     (Simulation.Definitions.compile ATC_Refinement
+        (@lift_L2 AuthenticationOperation _ TD _ (File.extend_inner v2 inum)))
+     (Finished s2' (Some r2)) ->
+     inum < Inode.InodeAllocatorParams.num_of_blocks ->
+   length (dedup_last addr_dec (rev (map fst (fst (snd s1'))))) =
+   length (dedup_last addr_dec (rev (map fst (fst (snd s2'))))) /\
+   (Forall (fun a : nat => a < data_length)
+      (map fst (fst (snd s1'))) <->
+    Forall (fun a : nat => a < data_length)
+      (map fst (fst (snd s2')))).
+      Proof.
+        Opaque File.extend_inner.
+       intros.
+       eapply_fresh refines_related_txn_empty in H; cleanup.
+       unfold AD_related_states, refines_related in *; simpl in *;
+        unfold HC_refines in *; simpl in *;
+        unfold TransactionToTransactionalDisk.Definitions.refines in *;
+        logic_clean.
+       eapply extend_inner_commit_pre' in H0, H1; subst; eauto.
+       cleanup; simpl.
+       repeat cleanup_pairs; eauto.
+       pose proof file_blocks_fit_in_disk.
+       pose proof inodes_before_data.
+       unfold File.DiskAllocatorParams.bitmap_addr,
+       File.DiskAllocatorParams.num_of_blocks,
+       Inode.InodeAllocatorParams.bitmap_addr,
+       Inode.InodeAllocatorParams.num_of_blocks in *.
+       simpl.
+       destruct (addr_dec file_blocks_start (file_blocks_start + S x7)); try lia.
+       destruct (addr_dec (inode_blocks_start + S inum)
+       (file_blocks_start + S x7)); try lia.
+       destruct (addr_dec (inode_blocks_start + S inum)
+       file_blocks_start); try lia.
+       destruct (addr_dec file_blocks_start (file_blocks_start + S x4)); try lia.
+       destruct (addr_dec (inode_blocks_start + S inum)
+       (file_blocks_start + S x4)); try lia.
+       simpl; intuition eauto;
+       repeat constructor; lia.
+    Qed.
+
+
+    Lemma rev_repeat:
+       forall T n (t: T),
+       rev (repeat t n) = repeat t n.
+       Proof.
+        induction n; simpl; eauto.
+        intros; rewrite IHn.
+        rewrite repeat_cons; eauto.
+        Qed.
+
+        Lemma dedup_last_repeat_length:
+        forall n a,
+        n = 0 \/ length (dedup_last addr_dec (repeat a n)) = 1.
+        Proof.
+         induction n; eauto.
+         intros.
+         edestruct IHn; cleanup; simpl; eauto.
+         destruct (in_dec addr_dec a (repeat a n)); eauto.
+         destruct n; simpl in *; try tauto.
+         Qed.
+         
+
+    Theorem delete_inner_commit_pre:
+   forall u u' inum (s0 s3 : state ATCLang) (o : oracle' ATCCore)
+     (s1' s2' : LayerImplementation.state' ATCCore) 
+     r1 r2,
+   refines_related ATC_Refinement (AD_related_states u' None) s0 s3 ->
+   exec ATCLang u o s0
+     (Simulation.Definitions.compile ATC_Refinement
+        (@lift_L2 AuthenticationOperation _ TD _ (File.delete_inner inum)))
+     (Finished s1' (Some r1)) ->
+   exec ATCLang u o s3
+     (Simulation.Definitions.compile ATC_Refinement
+        (@lift_L2 AuthenticationOperation _ TD _ (File.delete_inner inum)))
+     (Finished s2' (Some r2)) ->
+     inum < Inode.InodeAllocatorParams.num_of_blocks ->
+   length (dedup_last addr_dec (rev (map fst (fst (snd s1'))))) =
+   length (dedup_last addr_dec (rev (map fst (fst (snd s2'))))) /\
+   (Forall (fun a : nat => a < data_length)
+      (map fst (fst (snd s1'))) <->
+    Forall (fun a : nat => a < data_length)
+      (map fst (fst (snd s2')))).
+      Proof.
+        Opaque File.extend_inner.
+       intros.
+       eapply_fresh refines_related_txn_empty in H; cleanup.
+       unfold AD_related_states, refines_related in *; simpl in *;
+        unfold HC_refines in *; simpl in *;
+        unfold TransactionToTransactionalDisk.Definitions.refines,
+        FileToFileDisk.Definitions.refines,
+        FD_related_states,
+        File.files_rep,
+        File.files_inner_rep in *;
+        logic_clean.
+       eapply delete_inner_commit_pre' in H0, H1; subst; eauto.
+       cleanup; simpl.
+       repeat cleanup_pairs; eauto.
+       pose proof file_blocks_fit_in_disk.
+       pose proof inodes_before_data.
+       unfold File.DiskAllocatorParams.bitmap_addr,
+       File.DiskAllocatorParams.num_of_blocks,
+       Inode.InodeAllocatorParams.bitmap_addr,
+       Inode.InodeAllocatorParams.num_of_blocks in *.
+       simpl.
+       repeat rewrite app_nil_r; simpl.
+       setoid_rewrite H20;
+       setoid_rewrite H23.
+       repeat rewrite dedup_last_length_not_in_tail_S.
+       repeat rewrite rev_repeat.
+       assert (A: length (Inode.block_numbers x12) = length (Inode.block_numbers x9)). {
+        eapply_fresh FileInnerSpecs.inode_exists_then_file_exists in H1;
+        eapply_fresh FileInnerSpecs.inode_exists_then_file_exists in H0;
+        eauto; cleanup.
+        unfold File.file_map_rep in *; cleanup.
+        edestruct H13; eauto.
+        edestruct H7; eauto.
+        cleanup.
+        edestruct H8; logic_clean.
+        edestruct H29; eauto.
+        lia.
+       }
+        setoid_rewrite A;
+        intuition eauto.
+        all: intros Hin; apply in_rev, repeat_spec in Hin; lia.
+    Qed.
