src/Noninterference/LoggedDisk/ATCD_HSS.v
@@ -1,0 +1,2634 @@
+Require Import Eqdep Lia Lra Framework FSParameters FileDiskLayer. (* LoggedDiskLayer TransactionCacheLayer TransactionalDiskLayer. *)
+Require Import FileDiskNoninterference LoggedDiskRefinement.
+Require Import ATC_ORS HSS ATCDLayer ATCD_Simulation ATCD_AOE.
+Require Import LogCache_FinishedNotCrashed ATCD_ORS.
+Import FileDiskLayer.
+
+
+
+Lemma get_inode_compiled_same:
+forall u o s1 s1' r1 inum td1,
+Transaction.transaction_rep (snd s1) td1 ->
+exec ATCLang u o s1
+   (RefinementLift.compile
+      (HorizontalComposition AuthenticationOperation
+         TransactionCacheOperation)
+      (HorizontalComposition AuthenticationOperation
+         (TransactionalDiskLayer.TDCore data_length)) ATCLang AD
+      (HC_Core_Refinement ATCLang AD Definitions.TDCoreRefinement)
+      (option Inode.Inode)
+      (@lift_L2 AuthenticationOperation _ TD _ (Inode.get_inode inum)))
+   (Finished s1' r1) ->
+   s1 = s1'.
+   Proof.
+    Transparent Inode.get_inode.
+    unfold Inode.get_inode, Inode.InodeAllocator.read.
+    intros; cleanup; simpl in *; repeat invert_exec;
+    simpl in *; repeat invert_exec; eauto;
+    eapply Transaction.read_finished in H4; eauto;
+    cleanup; eauto;
+    repeat cleanup_pairs; eauto;
+    eapply Transaction.read_finished in H2; eauto;
+    cleanup; eauto.
+    Opaque Inode.get_inode.
+  Qed.
+
+Lemma disk_allocator_alloc_exact_txn:
+  forall u o s1 s1' r v1 td1,
+  Transaction.transaction_rep (snd s1) td1 ->
+exec ATCLang u o s1
+  (RefinementLift.compile
+     (HorizontalComposition AuthenticationOperation
+        TransactionCacheOperation)
+     (HorizontalComposition AuthenticationOperation
+        (TransactionalDiskLayer.TDCore data_length)) ATCLang AD
+     (HC_Core_Refinement ATCLang AD Definitions.TDCoreRefinement)
+     (option nat)
+     (@lift_L2 AuthenticationOperation _ TD _ (File.DiskAllocator.alloc v1)))
+  (Finished s1' r) ->
+     (r = None) \/ 
+     (exists v new_bitmap, 
+     r = Some v /\ 
+     fst (snd s1') = (File.DiskAllocatorParams.bitmap_addr, new_bitmap) :: (File.DiskAllocatorParams.bitmap_addr + S v, v1) :: fst (snd s1) /\
+     snd (snd s1') = snd (snd s1) /\
+     v < File.DiskAllocatorParams.num_of_blocks).
+     Proof.
+      Transparent File.DiskAllocator.alloc.
+      unfold File.DiskAllocator.alloc.
+      intros; cleanup; simpl in *; repeat invert_exec;
+      simpl in *; repeat invert_exec; eauto;
+      eapply Transaction.read_finished in H3; eauto;
+      cleanup; eauto.
+      {
+        repeat cleanup_pairs; eauto;
+        split_ors; cleanup; try lia.
+        eapply Transaction.write_finished in H5; eauto;
+        cleanup; eauto;
+        repeat split_ors; cleanup; try congruence.
+        simpl in *; repeat invert_exec;
+        simpl in *;
+        eapply Transaction.write_finished in H6; eauto.
+        repeat cleanup_pairs; eauto;
+        split_ors; cleanup; try lia;
+        simpl in *; repeat invert_exec.
+
+        right.
+        do 2 eexists; intuition eauto.
+
+        simpl in *; repeat invert_exec.
+        repeat cleanup_pairs; eauto.
+
+        pose proof File.DiskAllocatorParams.blocks_fit_in_disk.
+        unfold File.DiskAllocatorParams.bitmap_addr in *; lia.
+      }
+      {
+        simpl in *; repeat invert_exec.
+        repeat cleanup_pairs; eauto.
+      }
+      Opaque File.DiskAllocator.alloc.
+    Qed.
+
+
+Lemma diskallocator_free_exact_txn:
+    forall u o s1 s1' r v1 td1,
+    Transaction.transaction_rep (snd s1) td1 ->
+exec ATCLang u o s1
+    (RefinementLift.compile
+       (HorizontalComposition AuthenticationOperation
+          TransactionCacheOperation)
+       (HorizontalComposition AuthenticationOperation
+          (TransactionalDiskLayer.TDCore data_length)) ATCLang AD
+       (HC_Core_Refinement ATCLang AD Definitions.TDCoreRefinement)
+       (option unit)
+       (@lift_L2 AuthenticationOperation _ TD _ (File.DiskAllocator.free v1)))
+    (Finished s1' r) ->
+       (r = None) \/ 
+       (exists new_bitmap, 
+       r = Some tt /\ 
+       fst (snd s1') = (File.DiskAllocatorParams.bitmap_addr, new_bitmap) :: fst (snd s1) /\
+       snd (snd s1') = snd (snd s1)).
+       Proof.
+        Transparent File.DiskAllocator.free.
+        unfold File.DiskAllocator.free.
+        intros; cleanup; simpl in *; repeat invert_exec;
+        simpl in *; repeat invert_exec; eauto;
+        eapply Transaction.read_finished in H3; eauto;
+        cleanup; eauto.
+        {
+          repeat cleanup_pairs; eauto;
+          split_ors; cleanup; try lia.
+          eapply Transaction.write_finished in H5; eauto;
+          cleanup; eauto;
+          repeat split_ors; cleanup; try congruence.
+          simpl in *; repeat invert_exec;
+          simpl in *; eauto.
+          eauto.
+
+          pose proof File.DiskAllocatorParams.blocks_fit_in_disk.
+          unfold File.DiskAllocatorParams.bitmap_addr in *; lia.
+        }
+        Opaque File.DiskAllocator.free.
+      Qed.
+
+
+Lemma inode_allocator_alloc_exact_txn:
+forall u o s1 s1' r v1 td1,
+Transaction.transaction_rep (snd s1) td1 ->
+exec ATCLang u o s1
+(RefinementLift.compile
+(HorizontalComposition AuthenticationOperation
+TransactionCacheOperation)
+(HorizontalComposition AuthenticationOperation
+(TransactionalDiskLayer.TDCore data_length)) ATCLang AD
+(HC_Core_Refinement ATCLang AD Definitions.TDCoreRefinement)
+(option nat)
+(@lift_L2 AuthenticationOperation _ TD _ (Inode.InodeAllocator.alloc v1)))
+(Finished s1' r) ->
+(r = None) \/ 
+(exists v new_bitmap, 
+r = Some v /\ 
+fst (snd s1') = (Inode.InodeAllocatorParams.bitmap_addr, new_bitmap) :: (Inode.InodeAllocatorParams.bitmap_addr + S v, v1) :: fst (snd s1) /\
+snd (snd s1') = snd (snd s1) /\
+v < Inode.InodeAllocatorParams.num_of_blocks).
+Proof.
+Transparent Inode.InodeAllocator.alloc.
+unfold Inode.InodeAllocator.alloc.
+intros; cleanup; simpl in *; repeat invert_exec;
+simpl in *; repeat invert_exec; eauto;
+eapply Transaction.read_finished in H3; eauto;
+cleanup; eauto.
+{
+repeat cleanup_pairs; eauto;
+split_ors; cleanup; try lia.
+eapply Transaction.write_finished in H5; eauto;
+cleanup; eauto;
+repeat split_ors; cleanup; try congruence.
+simpl in *; repeat invert_exec;
+simpl in *;
+eapply Transaction.write_finished in H6; eauto.
+repeat cleanup_pairs; eauto;
+split_ors; cleanup; try lia;
+simpl in *; repeat invert_exec.
+
+right.
+do 2 eexists; intuition eauto.
+
+simpl in *; repeat invert_exec.
+repeat cleanup_pairs; eauto.
+
+pose proof Inode.InodeAllocatorParams.blocks_fit_in_disk.
+unfold Inode.InodeAllocatorParams.bitmap_addr in *; lia.
+}
+{
+simpl in *; repeat invert_exec.
+repeat cleanup_pairs; eauto.
+}
+Opaque Inode.InodeAllocator.alloc.
+Qed.
+
+
+Lemma free_all_blocks_exact_txn:
+forall u l o s1 s1' r td1,
+Transaction.transaction_rep (snd s1) td1 ->
+exec ATCLang u o s1
+(RefinementLift.compile
+(HorizontalComposition AuthenticationOperation
+TransactionCacheOperation)
+(HorizontalComposition AuthenticationOperation
+(TransactionalDiskLayer.TDCore data_length)) ATCLang AD
+(HC_Core_Refinement ATCLang AD Definitions.TDCoreRefinement)
+(option unit)
+(@lift_L2 AuthenticationOperation _ TD _ (File.free_all_blocks l)))
+(Finished s1' r) ->
+(r = None) \/ 
+(exists l', 
+r = Some tt /\ 
+fst (snd s1') = l' ++ fst (snd s1) /\
+snd (snd s1') = snd (snd s1) /\
+length l' = length l /\
+map fst l' = repeat File.DiskAllocatorParams.bitmap_addr (length l)).
+Proof.
+  induction l; 
+intros; cleanup; simpl in *; repeat invert_exec;
+simpl in *; repeat invert_exec; eauto.
+right; exists []; intuition eauto.
+
+eapply_fresh diskallocator_free_exact_txn in H0; eauto.
+eapply_fresh ATC_Simulation.ATC_oracle_refines_finished in H0; eauto.
+cleanup.
+eapply_fresh ATC_Simulation.ATC_exec_lift_finished in H0; eauto;
+try solve [apply TransactionToTransactionalDisk.Refinement.TC_to_TD_core_simulation_finished];
+cleanup.
+unfold Simulation.Definitions.refines in *; simpl in *.
+unfold HC_refines in *; simpl in *.
+unfold TransactionToTransactionalDisk.Definitions.refines in *; cleanup.
+
+split_ors; cleanup; try congruence.
+eapply IHl in H1; eauto.
+split_ors; cleanup; eauto.
+right; exists (x5 ++ [(File.DiskAllocatorParams.bitmap_addr, x4)]);
+intuition eauto.
+rewrite <- app_assoc; eauto.
+rewrite app_length; simpl; eauto.
+lia.
+
+repeat rewrite map_app.
+rewrite repeat_cons.
+simpl; eauto.
+rewrite H9; eauto.
+
+simpl.
+instantiate (1:= (_,_)).
+unfold HC_refines in *; simpl in *.
+unfold TransactionToTransactionalDisk.Definitions.refines in *; cleanup.
+intuition eauto.
+eexists (_, _).
+unfold HC_refines in *; simpl in *.
+unfold TransactionToTransactionalDisk.Definitions.refines in *; cleanup.
+intuition eauto.
+Unshelve.
+exact id.
+Qed.
+
+(**XXXXXXXXX**)
+
+Theorem ATC_HSS_transaction_recover:
+forall u s1 s2 o1 o2 o3 o4,
+((exists s1' s2' r1 r2,
+exec ATCLang u o1 s1 (@lift_L2 AuthenticationOperation _ TransactionCacheLang _ Transaction.recover) (Finished s1' r1) /\
+exec ATCLang u o2 s2 (@lift_L2 AuthenticationOperation _ TransactionCacheLang _ Transaction.recover) (Finished s2' r2)) \/
+(exists s1' s2',
+exec ATCLang u o1 s1 (@lift_L2 AuthenticationOperation _ TransactionCacheLang _ Transaction.recover) (Crashed s1') /\
+exec ATCLang u o2 s2 (@lift_L2 AuthenticationOperation _ TransactionCacheLang _ Transaction.recover) (Crashed s2'))) ->
+o1 ++ o3 = o2 ++ o4 -> 
+ATC_have_same_structure
+  (@lift_L2 AuthenticationOperation _ TransactionCacheLang _ Transaction.recover)
+  (@lift_L2 AuthenticationOperation _ TransactionCacheLang _ Transaction.recover) u s1 s2.
+Proof.
+  unfold Transaction.recover; intros.
+  split_ors; cleanup.
+  {
+    repeat (repeat invert_exec; cleanup).
+    all: try solve [simpl in *; cleanup].
+    {
+      repeat rewrite map_app;
+      do 4 eexists; intuition eauto.
+    }
+  }
+  {
+    repeat (repeat invert_exec; simpl in *; cleanup);
+    simpl; intuition eauto;
+    repeat invert_exec; simpl in *; cleanup;
+    simpl; eauto.
+  }
+Qed.
+
+Theorem ATC_HSS_transaction_commit:
+forall u s1 s2,
+let p1 := (@lift_L2 AuthenticationOperation _ TransactionCacheLang _ (Transaction.commit)) in
+let p2 := (@lift_L2 AuthenticationOperation _ TransactionCacheLang _ (Transaction.commit)) in
+(length (dedup_last addr_dec (rev (map fst (fst (snd s1))))) =
+length (dedup_last addr_dec (rev (map fst (fst (snd s2)))))) ->
+(Forall (fun a : nat => a < data_length) (map fst (fst (snd s1))) <->
+Forall (fun a : nat => a < data_length) (map fst (fst (snd s2)))) ->
+ATC_have_same_structure p1 p2 u s1 s2.
+Proof.
+  unfold Transaction.commit; simpl; intros; cleanup.
+  simpl in *; cleanup; intuition eauto;
+  repeat invert_exec.
+  eauto.
+  repeat rewrite <- dedup_last_dedup_by_list_length_le; eauto;
+  repeat rewrite rev_length, map_length; eauto.
+  eapply Transaction.dedup_last_NoDup.
+  eapply Transaction.dedup_last_NoDup.
+  eapply Forall_forall; intros.
+  apply Transaction.dedup_last_in, in_rev in H0.
+  eapply Forall_forall in H1; eauto.
+  eapply Forall_forall; intros.
+  eapply in_rev, Transaction.dedup_last_in in H5.
+  eapply Forall_forall in H4; eauto.
+
+  eapply Forall_forall; intros.
+  apply Transaction.dedup_last_in, in_rev in H0.
+  eapply Forall_forall in H2; eauto.
+  eapply Forall_forall; intros.
+  eapply in_rev, Transaction.dedup_last_in in H5.
+  eapply Forall_forall in H4; eauto.
+Qed.
+
+Theorem ATC_HSS_transaction_abort:
+forall u s1 s2,
+let p1 := (@lift_L2 AuthenticationOperation _ TransactionCacheLang _ (Transaction.abort)) in
+let p2 := (@lift_L2 AuthenticationOperation _ TransactionCacheLang _ (Transaction.abort)) in
+ATC_have_same_structure p1 p2 u s1 s2.
+Proof.
+  unfold Transaction.commit; simpl; intros; cleanup.
+  simpl in *; cleanup; intuition eauto;
+  repeat invert_exec.
+Qed.
+
+
+Theorem ATC_HSS_transaction_read:
+forall u s1 s2 a a0,
+let p1 := (@lift_L2 AuthenticationOperation _ TransactionCacheLang _ (Transaction.read a)) in
+let p2 := (@lift_L2 AuthenticationOperation _ TransactionCacheLang _ (Transaction.read a0)) in
+(a < data_length <-> a0 < data_length) ->
+(Transaction.get_first (fst (snd s1)) a = None <->  
+Transaction.get_first (fst (snd s2)) a0 = None) -> 
+ATC_have_same_structure p1 p2 u s1 s2.
+Proof.
+  unfold Transaction.read; simpl; intros; cleanup.
+  destruct (Compare_dec.lt_dec a data_length); 
+  destruct (Compare_dec.lt_dec a0 data_length); 
+  simpl; eauto; try lia.
+  simpl in *; cleanup; intuition eauto.
+  repeat invert_exec.
+  destruct_fresh (Transaction.get_first (fst (snd s1)) a);
+  destruct_fresh (Transaction.get_first (fst (snd s2)) a0);
+  simpl; try solve [intuition congruence];
+  setoid_rewrite D; setoid_rewrite D0; simpl; intuition eauto.
+Qed.
+
+Theorem ATC_HSS_transaction_write:
+forall u s1 s2 a a0 v v0, 
+let p1 := (@lift_L2 AuthenticationOperation _ TransactionCacheLang _ (Transaction.write a v)) in
+let p2 := (@lift_L2 AuthenticationOperation _ TransactionCacheLang _ (Transaction.write a0 v0)) in
+(a < data_length <-> a0 < data_length) ->
+((length (addr_list_to_blocks (map fst (fst (snd s1)) ++ [a])) +
+ length (map snd (fst (snd s1)) ++ [v])) <= log_length <->  
+ (length (addr_list_to_blocks (map fst (fst (snd s2)) ++ [a0])) +
+  length (map snd (fst (snd s2)) ++ [v0])) <= log_length) -> 
+ATC_have_same_structure p1 p2 u s1 s2.
+Proof.
+  unfold Transaction.write; simpl; intros; cleanup.
+  destruct (Compare_dec.lt_dec a data_length); 
+  destruct (Compare_dec.lt_dec a0 data_length); 
+  simpl; eauto; try lia.
+  simpl in *; cleanup; intuition eauto.
+  repeat invert_exec.
+  destruct_fresh (Compare_dec.le_dec
+  (length (addr_list_to_blocks (map fst (fst (snd s1)) ++ [a])) +
+   length (map snd (fst (snd s1)) ++ [v])) log_length);
+  destruct_fresh (Compare_dec.le_dec
+  (length (addr_list_to_blocks (map fst (fst (snd s2)) ++ [a0])) +
+   length (map snd (fst (snd s2)) ++ [v0])) log_length);
+  simpl; try solve [intuition lia];
+  setoid_rewrite D; setoid_rewrite D0; simpl; intuition eauto.
+Qed.
+
+Theorem ATC_HSS_inodeallocator_read:
+forall u inum s1 s2 td1 td2 im1 im2 fm1 fm2 u' ex bm1 bm2,
+let p1 := (@lift_L2 AuthenticationOperation _ TD _ (Inode.InodeAllocator.read inum)) in
+let p2 := (@lift_L2 AuthenticationOperation _ TD _ (Inode.InodeAllocator.read inum)) in
+(Transaction.get_first (fst (snd s1)) Inode.InodeAllocatorParams.bitmap_addr =
+None <->
+Transaction.get_first (fst (snd s2)) Inode.InodeAllocatorParams.bitmap_addr =
+None) ->
+(Transaction.get_first (fst (snd s1)) (Inode.InodeAllocatorParams.bitmap_addr + S inum) =
+None <->
+Transaction.get_first (fst (snd s2)) (Inode.InodeAllocatorParams.bitmap_addr + S inum) =
+None) ->
+
+Inode.inode_rep im1 (fst (snd td1)) ->
+Inode.inode_rep im2 (fst (snd td2)) ->
+File.file_map_rep fm1 im1 bm1 ->
+File.file_map_rep fm2 im2 bm2 ->
+same_for_user_except u' ex fm1 fm2 ->
+Transaction.transaction_rep (snd s1) td1 ->
+Transaction.transaction_rep (snd s2) td2 ->
+ATC_have_same_structure (ATC_Refinement.(Simulation.Definitions.compile) p1) 
+(ATC_Refinement.(Simulation.Definitions.compile) p2) u s1 s2.
+Proof.
+  unfold Inode.InodeAllocator.read; simpl; intros; cleanup.
+  destruct (Compare_dec.lt_dec inum Inode.InodeAllocatorParams.num_of_blocks); 
+  simpl; eauto.
+  simpl in *; cleanup; intuition eauto.
+  eapply ATC_HSS_transaction_read; try solve [intuition eauto].
+  eapply lift2_invert_exec in H0, H11; cleanup.
+  unfold  refines_related in *; simpl in *.
+  unfold HC_refines in *; simpl in *.
+  unfold TransactionToTransactionalDisk.Definitions.refines in *; simpl in *.
+  eapply Transaction.read_finished in H13, H15; eauto.
+  cleanup; repeat split_ors; cleanup; try lia.
+  
+  unfold AD_related_states, FD_related_states,
+  refines_related in *; simpl in *.
+  erewrite BlockAllocatorExistence.inode_allocations_are_same_2; eauto.
+  destruct_fresh (test_bit inum
+  (value_to_bits
+     (fst (snd td2) Inode.InodeAllocatorParams.bitmap_addr))).
+
+  simpl.
+
+  simpl in *; cleanup; intuition eauto.
+  eapply ATC_HSS_transaction_read; try solve [intuition eauto].
+  repeat cleanup_pairs; simpl; intuition eauto.
+  simpl; intuition eauto.
+  repeat rewrite block_allocator_empty; simpl; eauto.
+  Unshelve.
+Qed.
+
+Set Nested Proofs Allowed.
+Lemma refines_related_get_first_none:
+  forall u' ex s1 s2 i1 i2,
+  refines_related ATC_Refinement (AD_related_states u' ex) s1 s2 ->
+  Transaction.get_first (fst (snd s1)) i1 = None <->
+  Transaction.get_first (fst (snd s2)) i2 = None.
+Proof.
+  unfold refines_related in *; simpl in *.
+unfold HC_refines in *; simpl in *.
+unfold TransactionToTransactionalDisk.Definitions.refines in *; simpl in *.
+intros.
+unfold Transaction.transaction_rep in *; simpl in *.
+
+unfold AD_related_states, FD_related_states,
+refines_related in *; simpl in *.
+unfold FileToFileDisk.Definitions.refines,
+File.files_rep, File.files_inner_rep in *;
+logic_clean.
+repeat cleanup_pairs.
+repeat split_ors; cleanup; try congruence.
+repeat rewrite map_length in *;
+destruct s, s0; simpl in *; eauto; try lia.
+intuition eauto.
+Qed.
+
+  Theorem ATC_HSS_diskallocator_read:
+  forall u u' ex (s1 s2: state ATCLang) a a0,
+  let p1 := (@lift_L2 AuthenticationOperation _ TD _ (File.DiskAllocator.read a)) in
+  let p2 := (@lift_L2 AuthenticationOperation _ TD _ (File.DiskAllocator.read a0)) in
+  (a < File.DiskAllocatorParams.num_of_blocks <-> 
+  a0 < File.DiskAllocatorParams.num_of_blocks) ->
+  test_bit a
+            (value_to_bits
+               ((snd (snd s1)) File.DiskAllocatorParams.bitmap_addr)) =
+  test_bit a0
+            (value_to_bits
+               ((snd (snd s2)) File.DiskAllocatorParams.bitmap_addr)) ->
+  refines_related ATC_Refinement (AD_related_states u' ex) s1 s2 ->
+  ATC_have_same_structure (ATC_Refinement.(Simulation.Definitions.compile) p1) 
+  (ATC_Refinement.(Simulation.Definitions.compile) p2) u s1 s2.
+  Proof.
+    unfold File.DiskAllocator.read; simpl; intros; cleanup.
+    destruct (Compare_dec.lt_dec a File.DiskAllocatorParams.num_of_blocks); 
+    destruct (Compare_dec.lt_dec a0 File.DiskAllocatorParams.num_of_blocks); 
+    try lia; simpl; eauto.
+    simpl in *; cleanup; intuition eauto.
+    eapply ATC_HSS_transaction_read; try solve [intuition eauto].
+    eapply refines_related_get_first_none; eauto.
+
+    eapply lift2_invert_exec in H3, H4; cleanup.
+    unfold  refines_related in *; simpl in *.
+    unfold HC_refines in *; simpl in *.
+    unfold TransactionToTransactionalDisk.Definitions.refines in *; simpl in *.
+    logic_clean.
+    eapply Transaction.read_finished in H6, H8; eauto.
+    cleanup; repeat split_ors; cleanup; try lia.
+    repeat cleanup_pairs; cleanup.
+
+    unfold Transaction.transaction_rep in *; simpl in *.
+    
+    unfold AD_related_states, FD_related_states,
+    refines_related in *; simpl in *.
+    unfold FileToFileDisk.Definitions.refines,
+    File.files_rep, File.files_inner_rep in *;
+    logic_clean.
+    simpl in *; cleanup.
+    destruct_fresh (test_bit a0
+            (value_to_bits
+               (snd (snd s0) File.DiskAllocatorParams.bitmap_addr)));
+    simpl in *; cleanup; eauto.
+    repeat split; eauto.
+    eapply ATC_HSS_transaction_read; try solve [intuition eauto].
+    pose proof File.DiskAllocatorParams.blocks_fit_in_disk.
+    unfold File.DiskAllocatorParams.bitmap_addr,
+    File.DiskAllocatorParams.num_of_blocks in *; 
+    lia.
+
+    simpl; repeat split_ors; cleanup; try congruence.
+    repeat rewrite map_length in *; destruct s2, s4;
+    simpl in *; try lia.
+    intuition eauto.
+    repeat rewrite block_allocator_empty; simpl; eauto.
+    Unshelve.
+    Qed.
+
+
+    Theorem ATC_HSS_inodeallocator_alloc:
+    forall u u' ex (s1 s2: state ATCLang) v v0,
+    let p1 := (@lift_L2 AuthenticationOperation _ TD _ (Inode.InodeAllocator.alloc v)) in
+    let p2 := (@lift_L2 AuthenticationOperation _ TD _ (Inode.InodeAllocator.alloc v0)) in
+    refines_related ATC_Refinement (AD_related_states u' ex) s1 s2 ->
+    ATC_have_same_structure (ATC_Refinement.(Simulation.Definitions.compile) p1) 
+    (ATC_Refinement.(Simulation.Definitions.compile) p2) u s1 s2.
+    Proof.
+      Transparent Inode.InodeAllocator.alloc.
+      unfold Inode.InodeAllocator.alloc; simpl; intros; cleanup.
+      simpl in *; cleanup; intuition eauto.
+      eapply ATC_HSS_transaction_read; try solve [intuition eauto].
+      eapply refines_related_get_first_none; eauto.
+
+      eapply lift2_invert_exec in H0, H1; cleanup.
+      unfold refines_related in *; simpl in *.
+      unfold HC_refines in *; simpl in *.
+      unfold TransactionToTransactionalDisk.Definitions.refines in *; simpl in *;
+      cleanup.
+      eapply Transaction.read_finished in H3, H5; eauto.
+      cleanup; repeat split_ors; cleanup; try lia.
+      2: { pose proof Inode.InodeAllocatorParams.blocks_fit_in_disk.
+      unfold Inode.InodeAllocatorParams.bitmap_addr,
+      Inode.InodeAllocatorParams.num_of_blocks in *; 
+      lia. 
+      }
+      repeat cleanup_pairs; cleanup.
+      
+      unfold AD_related_states, FD_related_states,
+      refines_related in *; simpl in *.
+      unfold FileToFileDisk.Definitions.refines,
+      File.files_rep in *;
+      logic_clean.
+      simpl in *; cleanup.
+      eapply_fresh BlockAllocatorExistence.free_block_exists_iff_inode in H4; eauto.
+      destruct (Compare_dec.lt_dec
+      (get_first_zero_index
+         (value_to_bits (snd (snd s3) Inode.InodeAllocatorParams.bitmap_addr)))
+         Inode.InodeAllocatorParams.num_of_blocks);
+      destruct (Compare_dec.lt_dec
+      (get_first_zero_index
+         (value_to_bits (snd (snd s0) Inode.InodeAllocatorParams.bitmap_addr)))
+         Inode.InodeAllocatorParams.num_of_blocks);
+      try lia.
+
+      assert (A: length
+      (addr_list_to_blocks
+         (map fst (fst s4) ++
+          [Inode.InodeAllocatorParams.bitmap_addr +
+           S
+             (get_first_zero_index
+                (value_to_bits (snd (snd s3) Inode.InodeAllocatorParams.bitmap_addr)))])) +
+    length (map snd (fst s4) ++ [v]) <= log_length <->
+    length
+      (addr_list_to_blocks
+         (map fst (fst s5) ++
+          [Inode.InodeAllocatorParams.bitmap_addr +
+           S
+             (get_first_zero_index
+                (value_to_bits (snd (snd s0) Inode.InodeAllocatorParams.bitmap_addr)))])) +
+    length (map snd (fst s5) ++ [v0]) <= log_length). {
+        simpl.
+        repeat cleanup_pairs; simpl in *.
+        unfold TransactionToTransactionalDisk.Definitions.refines, AD_related_states, FD_related_states,
+        refines_related in *; simpl in *.
+        repeat cleanup_pairs; simpl in *.
+        
+        unfold Transaction.transaction_rep in *;
+        logic_clean; simpl in *.
+        repeat cleanup_pairs; simpl in *.
+
+        repeat rewrite map_length in *;
+        destruct s0, s2; simpl in *; 
+        repeat split_ors; 
+        cleanup; try congruence; try lia.
+        {
+          erewrite addr_list_to_blocks_length_eq with (l_b := ([Inode.InodeAllocatorParams.bitmap_addr +
+          S (get_first_zero_index (value_to_bits (s1 Inode.InodeAllocatorParams.bitmap_addr)))])).
+          intuition eauto.
+          simpl; eauto. 
+        }
+      }
+
+      simpl; intuition eauto.
+      eapply ATC_HSS_transaction_write.
+      {
+        repeat cleanup_pairs; simpl in *.
+        pose proof Inode.InodeAllocatorParams.blocks_fit_in_disk.
+        unfold Inode.InodeAllocatorParams.bitmap_addr,
+        Inode.InodeAllocatorParams.num_of_blocks in *; 
+        lia.
+      }
+      {
+        simpl; intuition eauto.
+      }
+
+      eapply lift2_invert_exec in H11, H15; cleanup.
+      unfold refines_related in *; simpl in *.
+      unfold HC_refines in *; simpl in *.
+      eapply Transaction.write_finished in H17, H19; eauto.
+      cleanup; repeat split_ors; cleanup; try lia.
+      {
+        simpl; intuition eauto.
+        eapply ATC_HSS_transaction_write.
+        intuition.
+        {
+          repeat cleanup_pairs; simpl in *.
+          unfold Transaction.transaction_rep in *;
+          logic_clean; simpl in *.
+          repeat cleanup_pairs; simpl in *.
+
+          repeat (split_ors; cleanup; try congruence; try lia).
+          repeat rewrite map_length in *;
+          destruct s, s2; simpl in *; try lia.
+          {
+              erewrite addr_list_to_blocks_length_eq with (l_b := ([Inode.InodeAllocatorParams.bitmap_addr +
+              S
+                (get_first_zero_index
+                  (value_to_bits (s4 Inode.InodeAllocatorParams.bitmap_addr)));
+                  Inode.InodeAllocatorParams.bitmap_addr])).
+              intuition eauto.
+              simpl; eauto. 
+          }
+        }
+        destruct r1, r2;
+        try destruct u0;
+        try destruct u1; simpl; eauto.
+      }
+      {
+        split_ors; cleanup.
+        
+        pose proof Inode.InodeAllocatorParams.blocks_fit_in_disk.
+        unfold Inode.InodeAllocatorParams.bitmap_addr,
+        Inode.InodeAllocatorParams.num_of_blocks in *; 
+        lia.
+
+        exfalso; eapply PeanoNat.Nat.lt_nge; eauto.
+      }
+      {
+        split_ors; cleanup.
+        
+        pose proof Inode.InodeAllocatorParams.blocks_fit_in_disk.
+        unfold Inode.InodeAllocatorParams.bitmap_addr,
+        Inode.InodeAllocatorParams.num_of_blocks in *; 
+        lia.
+
+        exfalso; eapply PeanoNat.Nat.lt_nge; eauto.
+      }
+      simpl; eauto.
+      simpl; eauto.
+      Unshelve.
+      Opaque Inode.InodeAllocator.alloc.
+    Qed.
+
+
+    Theorem ATC_HSS_diskallocator_alloc:
+    forall u u' ex (s1 s2: state ATCLang) v v0,
+    let p1 := (@lift_L2 AuthenticationOperation _ TD _ (File.DiskAllocator.alloc v)) in
+    let p2 := (@lift_L2 AuthenticationOperation _ TD _ (File.DiskAllocator.alloc v0)) in
+    refines_related ATC_Refinement (AD_related_states u' ex) s1 s2 ->
+    ATC_have_same_structure (ATC_Refinement.(Simulation.Definitions.compile) p1) 
+    (ATC_Refinement.(Simulation.Definitions.compile) p2) u s1 s2.
+    Proof.
+      Transparent File.DiskAllocator.alloc.
+      unfold File.DiskAllocator.alloc; simpl; intros; cleanup.
+      simpl in *; cleanup; intuition eauto.
+      eapply ATC_HSS_transaction_read; try solve [intuition eauto].
+      eapply refines_related_get_first_none; eauto.
+
+      eapply lift2_invert_exec in H0, H1; cleanup.
+      unfold refines_related in *; simpl in *.
+      unfold HC_refines in *; simpl in *.
+      unfold TransactionToTransactionalDisk.Definitions.refines in *; simpl in *;
+      cleanup.
+      eapply Transaction.read_finished in H3, H5; eauto.
+      cleanup; repeat split_ors; cleanup; try lia.
+      2: { pose proof File.DiskAllocatorParams.blocks_fit_in_disk.
+      unfold File.DiskAllocatorParams.bitmap_addr,
+      File.DiskAllocatorParams.num_of_blocks in *; 
+      lia. 
+      }
+      repeat cleanup_pairs; cleanup.
+      
+      unfold AD_related_states, FD_related_states,
+      refines_related in *; simpl in *.
+      unfold FileToFileDisk.Definitions.refines,
+      File.files_rep in *;
+      logic_clean.
+      simpl in *; cleanup.
+      eapply_fresh BlockAllocatorExistence.free_block_exists_iff in H4; eauto.
+      destruct (Compare_dec.lt_dec
+      (get_first_zero_index
+         (value_to_bits (snd (snd s3) File.DiskAllocatorParams.bitmap_addr)))
+      File.DiskAllocatorParams.num_of_blocks);
+      destruct (Compare_dec.lt_dec
+      (get_first_zero_index
+         (value_to_bits (snd (snd s0) File.DiskAllocatorParams.bitmap_addr)))
+      File.DiskAllocatorParams.num_of_blocks);
+      try lia.
+
+      assert (A: length
+      (addr_list_to_blocks
+         (map fst (fst s4) ++
+          [File.DiskAllocatorParams.bitmap_addr +
+           S
+             (get_first_zero_index
+                (value_to_bits (snd (snd s3) File.DiskAllocatorParams.bitmap_addr)))])) +
+    length (map snd (fst s4) ++ [v]) <= log_length <->
+    length
+      (addr_list_to_blocks
+         (map fst (fst s5) ++
+          [File.DiskAllocatorParams.bitmap_addr +
+           S
+             (get_first_zero_index
+                (value_to_bits (snd (snd s0) File.DiskAllocatorParams.bitmap_addr)))])) +
+    length (map snd (fst s5) ++ [v0]) <= log_length). {
+        simpl.
+        repeat cleanup_pairs; simpl in *.
+        unfold TransactionToTransactionalDisk.Definitions.refines, AD_related_states, FD_related_states,
+        refines_related in *; simpl in *.
+        repeat cleanup_pairs; simpl in *.
+        
+        unfold Transaction.transaction_rep in *;
+        logic_clean; simpl in *.
+        repeat cleanup_pairs; simpl in *.
+
+        repeat rewrite map_length in *;
+        destruct s0, s2; simpl in *; 
+        repeat split_ors; 
+        cleanup; try congruence; try lia.
+        {
+          erewrite addr_list_to_blocks_length_eq with (l_b := ([File.DiskAllocatorParams.bitmap_addr +
+          S (get_first_zero_index (value_to_bits (s1 File.DiskAllocatorParams.bitmap_addr)))])).
+          intuition eauto.
+          simpl; eauto. 
+        }
+      }
+
+      simpl; intuition eauto.
+      eapply ATC_HSS_transaction_write.
+      {
+        repeat cleanup_pairs; simpl in *.
+        pose proof File.DiskAllocatorParams.blocks_fit_in_disk.
+        unfold File.DiskAllocatorParams.bitmap_addr,
+        File.DiskAllocatorParams.num_of_blocks in *; 
+        lia.
+      }
+      {
+        simpl; intuition eauto.
+      }
+
+      eapply lift2_invert_exec in H11, H15; cleanup.
+      unfold refines_related in *; simpl in *.
+      unfold HC_refines in *; simpl in *.
+      eapply Transaction.write_finished in H17, H19; eauto.
+      cleanup; repeat split_ors; cleanup; try lia.
+      {
+        simpl; intuition eauto.
+        eapply ATC_HSS_transaction_write.
+        intuition.
+        {
+          repeat cleanup_pairs; simpl in *.
+          unfold Transaction.transaction_rep in *;
+          logic_clean; simpl in *.
+          repeat cleanup_pairs; simpl in *.
+
+          repeat (split_ors; cleanup; try congruence; try lia).
+          repeat rewrite map_length in *;
+          destruct s, s2; simpl in *; try lia.
+          {
+              erewrite addr_list_to_blocks_length_eq with (l_b := ([File.DiskAllocatorParams.bitmap_addr +
+              S
+                (get_first_zero_index
+                  (value_to_bits (s4 File.DiskAllocatorParams.bitmap_addr)));
+            File.DiskAllocatorParams.bitmap_addr])).
+              intuition eauto.
+              simpl; eauto. 
+          }
+        }
+        destruct r1, r2;
+        try destruct u0;
+        try destruct u1; simpl; eauto.
+      }
+      {
+        split_ors; cleanup.
+        
+        pose proof File.DiskAllocatorParams.blocks_fit_in_disk.
+        unfold File.DiskAllocatorParams.bitmap_addr,
+        File.DiskAllocatorParams.num_of_blocks in *; 
+        lia.
+
+        exfalso; eapply PeanoNat.Nat.lt_nge; eauto.
+      }
+      {
+        split_ors; cleanup.
+        
+        pose proof File.DiskAllocatorParams.blocks_fit_in_disk.
+        unfold File.DiskAllocatorParams.bitmap_addr,
+        File.DiskAllocatorParams.num_of_blocks in *; 
+        lia.
+
+        exfalso; eapply PeanoNat.Nat.lt_nge; eauto.
+      }
+      simpl; eauto.
+      simpl; eauto.
+      Unshelve.
+      Opaque File.DiskAllocator.alloc.
+    Qed.
+
+    Theorem ATC_HSS_inodeallocator_write:
+    forall u (s1 s2: state ATCLang) a v v0 td1 td2,
+    let p1 := (@lift_L2 AuthenticationOperation _ TD _ (Inode.InodeAllocator.write a v)) in
+    let p2 := (@lift_L2 AuthenticationOperation _ TD _ (Inode.InodeAllocator.write a v0)) in
+    (Transaction.get_first (fst (snd s1)) Inode.InodeAllocatorParams.bitmap_addr =
+    None <->
+    Transaction.get_first (fst (snd s2)) Inode.InodeAllocatorParams.bitmap_addr =
+    None) ->
+    test_bit a
+              (value_to_bits
+                 ((fst (snd td1)) Inode.InodeAllocatorParams.bitmap_addr)) =
+    test_bit a
+              (value_to_bits
+                 ((fst (snd td2)) Inode.InodeAllocatorParams.bitmap_addr)) ->
+    Transaction.transaction_rep (snd s1) td1 ->
+    Transaction.transaction_rep (snd s2) td2 ->
+    (length
+    (addr_list_to_blocks
+       (map fst (fst (snd s1)) ++
+        [Inode.InodeAllocatorParams.bitmap_addr + S a])) +
+  length (map snd (fst (snd s1)) ++ [v]) <= log_length <->
+  length
+    (addr_list_to_blocks
+       (map fst (fst (snd s2)) ++
+        [Inode.InodeAllocatorParams.bitmap_addr + S a])) +
+  length (map snd (fst (snd s2)) ++ [v0]) <= log_length) ->
+    ATC_have_same_structure (ATC_Refinement.(Simulation.Definitions.compile) p1) 
+    (ATC_Refinement.(Simulation.Definitions.compile) p2) u s1 s2.
+    Proof.
+      unfold Inode.InodeAllocator.write; simpl; intros; cleanup.
+      destruct (Compare_dec.lt_dec a Inode.InodeAllocatorParams.num_of_blocks); 
+      try lia; simpl; eauto.
+      simpl in *; cleanup; intuition eauto.
+      eapply ATC_HSS_transaction_read; try solve [intuition eauto].
+      eapply lift2_invert_exec in H3, H7; cleanup.
+      unfold refines_related in *; simpl in *.
+      unfold HC_refines in *; simpl in *.
+      eapply Transaction.read_finished in H9, H11; eauto.
+      cleanup; repeat split_ors; cleanup; try lia.
+      setoid_rewrite H0.
+      destruct_fresh (test_bit a
+              (value_to_bits
+                 (fst (snd td2) Inode.InodeAllocatorParams.bitmap_addr)));
+      setoid_rewrite D;
+      simpl in *; cleanup; eauto.
+      repeat split; eauto.
+      eapply ATC_HSS_transaction_write; try solve [intuition eauto].
+      repeat cleanup_pairs; intuition eauto.
+      repeat rewrite block_allocator_empty; simpl; eauto.
+      Unshelve.
+      Qed.
+
+
+
+    Theorem ATC_HSS_diskallocator_write:
+    forall u (s1 s2: state ATCLang) a a0 v v0 td1 td2,
+    let p1 := (@lift_L2 AuthenticationOperation _ TD _ (File.DiskAllocator.write a v)) in
+    let p2 := (@lift_L2 AuthenticationOperation _ TD _ (File.DiskAllocator.write a0 v0)) in
+    (a < File.DiskAllocatorParams.num_of_blocks <-> 
+    a0 < File.DiskAllocatorParams.num_of_blocks) ->
+    test_bit a
+              (value_to_bits
+                 ((fst (snd td1)) File.DiskAllocatorParams.bitmap_addr)) =
+    test_bit a0
+              (value_to_bits
+                 ((fst (snd td2)) File.DiskAllocatorParams.bitmap_addr)) ->
+    (Transaction.get_first (fst (snd s1)) File.DiskAllocatorParams.bitmap_addr =
+    None <->
+    Transaction.get_first (fst (snd s2)) File.DiskAllocatorParams.bitmap_addr =
+    None) ->
+    (length
+    (addr_list_to_blocks
+       (map fst (fst (snd s1)) ++ [File.DiskAllocatorParams.bitmap_addr + S a])) +
+  length (map snd (fst (snd s1)) ++ [v]) <= log_length <->
+  length
+    (addr_list_to_blocks
+       (map fst (fst (snd s2)) ++ [File.DiskAllocatorParams.bitmap_addr + S a0])) +
+  length (map snd (fst (snd s2)) ++ [v0]) <= log_length) ->
+    Transaction.transaction_rep (snd s1) td1 ->
+    Transaction.transaction_rep (snd s2) td2 ->
+    ATC_have_same_structure (ATC_Refinement.(Simulation.Definitions.compile) p1) 
+    (ATC_Refinement.(Simulation.Definitions.compile) p2) u s1 s2.
+    Proof.
+      unfold File.DiskAllocator.write; simpl; intros; cleanup.
+      destruct (Compare_dec.lt_dec a File.DiskAllocatorParams.num_of_blocks); 
+      destruct (Compare_dec.lt_dec a0 File.DiskAllocatorParams.num_of_blocks); 
+      try lia; simpl; eauto.
+      simpl in *; cleanup; intuition eauto.
+      eapply ATC_HSS_transaction_read; try solve [intuition eauto].
+
+      eapply lift2_invert_exec in H6, H9; cleanup.
+      unfold refines_related in *; simpl in *.
+      unfold HC_refines in *; simpl in *.
+      eapply Transaction.read_finished in H11, H13; eauto.
+      cleanup; repeat split_ors; cleanup; try lia.
+      repeat cleanup_pairs; cleanup.
+      simpl; cleanup.
+      cleanup.
+      destruct_fresh (test_bit a0
+              (value_to_bits
+                 (v2 File.DiskAllocatorParams.bitmap_addr)));
+      simpl in *; cleanup; eauto.
+      repeat split; eauto.
+      eapply ATC_HSS_transaction_write; try solve [intuition eauto].
+      pose proof File.DiskAllocatorParams.blocks_fit_in_disk.
+      unfold File.DiskAllocatorParams.bitmap_addr,
+      File.DiskAllocatorParams.num_of_blocks in *; 
+      lia.
+      repeat rewrite block_allocator_empty; simpl; eauto.
+      Unshelve.
+      Qed.
+
+Theorem ATC_HSS_diskallocator_free:
+forall u (s1 s2: state ATCLang) a a0 td1 td2,
+let p1 := (@lift_L2 AuthenticationOperation _ TD _ (File.DiskAllocator.free a)) in
+let p2 := (@lift_L2 AuthenticationOperation _ TD _ (File.DiskAllocator.free a0)) in
+(a < File.DiskAllocatorParams.num_of_blocks <-> 
+a0 < File.DiskAllocatorParams.num_of_blocks) ->
+test_bit a
+          (value_to_bits
+              ((fst (snd td1)) File.DiskAllocatorParams.bitmap_addr)) =
+test_bit a0
+          (value_to_bits
+              ((fst (snd td2)) File.DiskAllocatorParams.bitmap_addr)) ->
+(Transaction.get_first (fst (snd s1)) File.DiskAllocatorParams.bitmap_addr =
+None <->
+Transaction.get_first (fst (snd s2)) File.DiskAllocatorParams.bitmap_addr =
+None) ->
+Transaction.transaction_rep (snd s1) td1 ->
+Transaction.transaction_rep (snd s2) td2 ->
+length (fst (snd s1)) = length (fst (snd s2)) ->
+ATC_have_same_structure (ATC_Refinement.(Simulation.Definitions.compile) p1) 
+(ATC_Refinement.(Simulation.Definitions.compile) p2) u s1 s2.
+Proof.
+  Transparent File.DiskAllocator.free.
+  unfold File.DiskAllocator.free; simpl; intros; cleanup.
+  destruct (Compare_dec.lt_dec a File.DiskAllocatorParams.num_of_blocks); 
+  destruct (Compare_dec.lt_dec a0 File.DiskAllocatorParams.num_of_blocks); 
+  try lia; simpl; eauto.
+  simpl in *; cleanup; intuition eauto.
+  eapply ATC_HSS_transaction_read; try solve [intuition eauto].
+
+  eapply lift2_invert_exec in H6, H8; cleanup.
+  unfold refines_related in *; simpl in *.
+  unfold HC_refines in *; simpl in *.
+  eapply Transaction.read_finished in H10, H12; eauto.
+  cleanup; repeat split_ors; cleanup; try lia.
+  repeat cleanup_pairs; cleanup.
+  simpl; cleanup.
+  cleanup.
+  destruct_fresh (test_bit a0
+          (value_to_bits
+              (v0 File.DiskAllocatorParams.bitmap_addr)));
+  simpl in *; cleanup; eauto.
+  repeat split; eauto.
+  eapply ATC_HSS_transaction_write; try solve [intuition eauto].
+  {
+    simpl.
+    repeat rewrite app_length, map_length; simpl.
+    erewrite addr_list_to_blocks_length_eq.
+    setoid_rewrite H4; intuition eauto.
+    repeat rewrite app_length, map_length; simpl; eauto.
+  }
+  repeat rewrite block_allocator_empty; simpl; eauto.
+  Unshelve.
+  Opaque File.DiskAllocator.free.
+  Qed.
+        
+
+  Theorem ATC_HSS_inodeallocator_free:
+  forall u (s1 s2: state ATCLang) a a0 td1 td2,
+  let p1 := (@lift_L2 AuthenticationOperation _ TD _ (Inode.InodeAllocator.free a)) in
+  let p2 := (@lift_L2 AuthenticationOperation _ TD _ (Inode.InodeAllocator.free a0)) in
+  (a < Inode.InodeAllocatorParams.num_of_blocks <-> 
+  a0 < Inode.InodeAllocatorParams.num_of_blocks) ->
+  test_bit a
+            (value_to_bits
+                ((fst (snd td1)) Inode.InodeAllocatorParams.bitmap_addr)) =
+  test_bit a0
+            (value_to_bits
+                ((fst (snd td2)) Inode.InodeAllocatorParams.bitmap_addr)) ->
+  (Transaction.get_first (fst (snd s1)) Inode.InodeAllocatorParams.bitmap_addr =
+  None <->
+  Transaction.get_first (fst (snd s2)) Inode.InodeAllocatorParams.bitmap_addr =
+  None) ->
+  Transaction.transaction_rep (snd s1) td1 ->
+  Transaction.transaction_rep (snd s2) td2 ->
+  length (fst (snd s1)) = length (fst (snd s2)) ->
+  ATC_have_same_structure (ATC_Refinement.(Simulation.Definitions.compile) p1) 
+  (ATC_Refinement.(Simulation.Definitions.compile) p2) u s1 s2.
+  Proof.
+    unfold Inode.InodeAllocator.free; simpl; intros; cleanup.
+    destruct (Compare_dec.lt_dec a Inode.InodeAllocatorParams.num_of_blocks); 
+    destruct (Compare_dec.lt_dec a0 Inode.InodeAllocatorParams.num_of_blocks); 
+    try lia; simpl; eauto.
+    simpl in *; cleanup; intuition eauto.
+    eapply ATC_HSS_transaction_read; try solve [intuition eauto].
+  
+    eapply lift2_invert_exec in H6, H8; cleanup.
+    unfold refines_related in *; simpl in *.
+    unfold HC_refines in *; simpl in *.
+    eapply Transaction.read_finished in H10, H12; eauto.
+    cleanup; repeat split_ors; cleanup; try lia.
+    repeat cleanup_pairs; cleanup.
+    simpl; cleanup.
+    cleanup.
+    destruct_fresh (test_bit a0
+            (value_to_bits
+                (v0 Inode.InodeAllocatorParams.bitmap_addr)));
+    simpl in *; cleanup; eauto.
+    repeat split; eauto.
+    eapply ATC_HSS_transaction_write; try solve [intuition eauto].
+    {
+      simpl.
+      repeat rewrite app_length, map_length; simpl.
+      erewrite addr_list_to_blocks_length_eq.
+      setoid_rewrite H4; intuition eauto.
+      repeat rewrite app_length, map_length; simpl; eauto.
+    }
+    repeat rewrite block_allocator_empty; simpl; eauto.
+    Unshelve.
+    Qed.
+
+
+  Theorem ATC_HSS_inode_get_inode:
+  forall u inum s1 s2 td1 td2 im1 im2 fm1 fm2 u' ex bm1 bm2,
+  let p1 := (@lift_L2 AuthenticationOperation _ TD _ (Inode.get_inode inum)) in
+  let p2 := (@lift_L2 AuthenticationOperation _ TD _ (Inode.get_inode inum)) in
+  
+  (Transaction.get_first (fst (snd s1)) Inode.InodeAllocatorParams.bitmap_addr =
+  None <->
+  Transaction.get_first (fst (snd s2)) Inode.InodeAllocatorParams.bitmap_addr =
+  None) ->
+  (Transaction.get_first (fst (snd s1)) (Inode.InodeAllocatorParams.bitmap_addr + S inum) =
+  None <->
+  Transaction.get_first (fst (snd s2)) (Inode.InodeAllocatorParams.bitmap_addr + S inum) =
+  None) ->
+  Inode.inode_rep im1 (fst (snd td1)) ->
+  Inode.inode_rep im2 (fst (snd td2)) ->
+  File.file_map_rep fm1 im1 bm1 ->
+  File.file_map_rep fm2 im2 bm2 ->
+  same_for_user_except u' ex fm1 fm2 ->
+  Transaction.transaction_rep (snd s1) td1 ->
+  Transaction.transaction_rep (snd s2) td2 ->
+  ATC_have_same_structure (ATC_Refinement.(Simulation.Definitions.compile) p1) 
+  (ATC_Refinement.(Simulation.Definitions.compile) p2) u s1 s2.
+  Proof.
+    Transparent Inode.get_inode.
+    unfold Inode.get_inode; simpl; intros; cleanup.
+    intuition eauto.
+    eapply ATC_HSS_inodeallocator_read. 
+    8: eauto.
+    8: eauto.
+    8: eauto.
+    all: try solve [intuition eauto].
+    destruct r1, r2; simpl; eauto.
+    Opaque Inode.get_inode.
+  Qed.
+
+
+  Theorem ATC_HSS_inode_set_inode:
+  forall u inum s1 s2 td1 td2 i1 i2,
+  let p1 := (@lift_L2 AuthenticationOperation _ TD _ (Inode.set_inode inum i1)) in
+  let p2 := (@lift_L2 AuthenticationOperation _ TD _ (Inode.set_inode inum i2)) in
+  
+  (Transaction.get_first (fst (snd s1)) Inode.InodeAllocatorParams.bitmap_addr =
+  None <->
+  Transaction.get_first (fst (snd s2)) Inode.InodeAllocatorParams.bitmap_addr =
+  None) ->
+  test_bit inum
+            (value_to_bits
+                ((fst (snd td1)) Inode.InodeAllocatorParams.bitmap_addr)) =
+  test_bit inum
+            (value_to_bits
+                ((fst (snd td2)) Inode.InodeAllocatorParams.bitmap_addr)) ->
+  (length
+  (addr_list_to_blocks
+     (map fst (fst (snd s1)) ++
+      [Inode.InodeAllocatorParams.bitmap_addr + S inum])) +
+length (map snd (fst (snd s1)) ++ [Inode.encode_inode i1]) <= log_length <->
+length
+  (addr_list_to_blocks
+     (map fst (fst (snd s2)) ++
+      [Inode.InodeAllocatorParams.bitmap_addr + S inum])) +
+length (map snd (fst (snd s2)) ++ [Inode.encode_inode i2]) <= log_length) ->
+  Transaction.transaction_rep (snd s1) td1 ->
+  Transaction.transaction_rep (snd s2) td2 ->
+  ATC_have_same_structure (ATC_Refinement.(Simulation.Definitions.compile) p1) 
+  (ATC_Refinement.(Simulation.Definitions.compile) p2) u s1 s2.
+  Proof.
+    unfold Inode.set_inode; simpl; intros; cleanup.
+    eapply ATC_HSS_inodeallocator_write. 
+    3: eauto.
+    3: eauto.
+    all: try solve [intuition eauto].
+    Opaque Inode.set_inode.
+  Qed.
+
+
+  Theorem ATC_HSS_inode_extend:
+  forall u inum s1 s2 td1 td2 im1 im2 fm1 fm2 u' ex bm1 bm2 bn1 bn2,
+  let p1 := (@lift_L2 AuthenticationOperation _ TD _ (Inode.extend inum bn1)) in
+  let p2 := (@lift_L2 AuthenticationOperation _ TD _ (Inode.extend inum bn2)) in
+  
+  (Transaction.get_first (fst (snd s1)) Inode.InodeAllocatorParams.bitmap_addr =
+  None <->
+  Transaction.get_first (fst (snd s2)) Inode.InodeAllocatorParams.bitmap_addr =
+  None) ->
+  (Transaction.get_first (fst (snd s1)) (Inode.InodeAllocatorParams.bitmap_addr + S inum) =
+  None <->
+  Transaction.get_first (fst (snd s2)) (Inode.InodeAllocatorParams.bitmap_addr + S inum) =
+  None) ->
+  Inode.inode_rep im1 (fst (snd td1)) ->
+  Inode.inode_rep im2 (fst (snd td2)) ->
+  File.file_map_rep fm1 im1 bm1 ->
+  File.file_map_rep fm2 im2 bm2 ->
+  same_for_user_except u' ex fm1 fm2 ->
+  Transaction.transaction_rep (snd s1) td1 ->
+  Transaction.transaction_rep (snd s2) td2 ->
+  length (fst (snd s1)) = length (fst (snd s2)) -> 
+  ATC_have_same_structure (ATC_Refinement.(Simulation.Definitions.compile) p1) 
+  (ATC_Refinement.(Simulation.Definitions.compile) p2) u s1 s2.
+  Proof.
+    Transparent Inode.extend.
+    unfold Inode.extend; simpl; intros; cleanup.
+    intuition eauto.
+    eapply ATC_HSS_inode_get_inode.
+    8: eauto. 
+    8: eauto. 
+    8: eauto.
+    all: try solve [intuition eauto].
+    unfold refines_related in *; simpl in *.
+    cleanup.
+    eapply_fresh get_inode_compiled_same in H0;
+    eapply_fresh get_inode_compiled_same in H12; eauto; cleanup.
+
+    eapply_fresh ATC_Simulation.ATC_oracle_refines_finished in H0;
+    eapply_fresh ATC_Simulation.ATC_oracle_refines_finished in H12; eauto.
+    cleanup.
+    eapply ATC_Simulation.ATC_exec_lift_finished in H0, H12; eauto;
+    try solve [apply TransactionToTransactionalDisk.Refinement.TC_to_TD_core_simulation_finished];
+    cleanup.
+    all: try instantiate (1:= (_, _)); simpl; unfold HC_refines; simpl;
+    unfold TransactionToTransactionalDisk.Definitions.refines; 
+    try split; eauto; try solve [eexists (_, _); intuition eauto].
+
+    eapply lift2_invert_exec in H0; cleanup.
+    eapply lift2_invert_exec in H12; cleanup.
+    unfold AD_related_states, FD_related_states,
+      refines_related in *; simpl in *.
+    eapply Inode.get_inode_finished_precise in H18; eauto.
+    eapply Inode.get_inode_finished_precise in H19; eauto.
+    cleanup.
+    repeat split_ors; cleanup.
+    repeat cleanup_pairs.
+    eapply ATC_HSS_inode_set_inode.
+    4: eauto.
+    4: eauto.
+    all: simpl; eauto.
+    {
+      unfold HC_refines in *; simpl in *.
+      unfold TransactionToTransactionalDisk.Definitions.refines,
+      Transaction.transaction_rep in *; simpl in *; cleanup.
+      intuition eauto.
+    }
+    {
+      eapply BlockAllocatorExistence.inode_allocations_are_same; eauto.
+      destruct H5.
+      unfold File.file_map_rep in *; logic_clean.
+      eapply BlockAllocatorExistence.addrs_match_exactly_trans; eauto.
+      eapply BlockAllocatorExistence.addrs_match_exactly_sym; eauto.
+      eapply BlockAllocatorExistence.addrs_match_exactly_trans; eauto.
+    }
+    {
+      repeat rewrite app_length, map_length; simpl.
+      erewrite addr_list_to_blocks_length_eq.
+      rewrite H8; intuition eauto.
+      repeat rewrite app_length, map_length; simpl; lia.
+    }
+      {
+        eapply FileInnerSpecs.inode_exists_then_file_exists in H19; eauto.
+        eapply FileInnerSpecs.inode_missing_then_file_missing in H21; eauto.
+        cleanup.
+        edestruct H5.
+        edestruct H18.
+        intuition; eauto.
+        exfalso; eapply H23; intuition eauto.
+        congruence.
+      }
+      {
+        eapply FileInnerSpecs.inode_exists_then_file_exists in H20; eauto.
+        eapply FileInnerSpecs.inode_missing_then_file_missing in H19; eauto.
+        cleanup.
+        edestruct H5.
+        edestruct H18.
+        intuition; eauto.
+        exfalso; eapply H22; intuition eauto.
+        congruence.
+      }
+      Unshelve.
+      all: exact id.
+      Opaque Inode.extend.
+    Qed.
+
+Theorem ATC_HSS_inode_get_block_number:
+forall u u' ex inum off s1 s2,
+let p1 := (@lift_L2 AuthenticationOperation _ TD _ (Inode.get_block_number inum off)) in
+let p2 := (@lift_L2 AuthenticationOperation _ TD _ (Inode.get_block_number inum off)) in
+
+refines_related ATC_Refinement (AD_related_states u' ex) s1 s2 ->
+ATC_have_same_structure (ATC_Refinement.(Simulation.Definitions.compile) p1) 
+(ATC_Refinement.(Simulation.Definitions.compile) p2) u s1 s2.
+Proof.
+  Transparent Inode.get_block_number.
+  unfold Inode.get_block_number; simpl; intros; cleanup.
+  intuition eauto.
+  unfold refines_related in *; simpl in *.
+  unfold HC_refines in *; simpl in *.
+  unfold TransactionToTransactionalDisk.Definitions.refines in *; simpl in *;
+  cleanup.
+  unfold AD_related_states, FD_related_states,
+  refines_related in *; simpl in *.
+  unfold FileToFileDisk.Definitions.refines,
+  File.files_rep, File.files_inner_rep in *;
+  logic_clean.
+  simpl in *; cleanup.
+  repeat cleanup_pairs.
+  eapply ATC_HSS_inode_get_inode.
+  7: eauto.
+  7: eauto.
+  7: eauto.
+  all: eauto.
+  eapply refines_related_get_first_none.
+  unfold refines_related in *; simpl in *.
+  unfold HC_refines in *; simpl in *.
+  unfold TransactionToTransactionalDisk.Definitions.refines in *; simpl in *;
+  cleanup.
+  unfold AD_related_states, FD_related_states,
+  refines_related in *; simpl in *.
+  unfold FileToFileDisk.Definitions.refines,
+  File.files_rep, File.files_inner_rep in *;
+  simpl in *; cleanup.
+  eexists (_, _), (_, _).
+  intuition eauto.
+  simpl; do 2 eexists; intuition eauto.
+
+  eapply refines_related_get_first_none.
+  unfold refines_related in *; simpl in *.
+  unfold HC_refines in *; simpl in *.
+  unfold TransactionToTransactionalDisk.Definitions.refines in *; simpl in *;
+  cleanup.
+  unfold AD_related_states, FD_related_states,
+  refines_related in *; simpl in *.
+  unfold FileToFileDisk.Definitions.refines,
+  File.files_rep, File.files_inner_rep in *;
+  simpl in *; cleanup.
+  eexists (_, _), (_, _).
+  intuition eauto.
+  simpl; do 2 eexists; intuition eauto.
+
+  destruct r1, r2; simpl; eauto.
+  Opaque Inode.get_block_number.
+Qed.
+
+
+Theorem ATC_HSS_inode_get_all_block_numbers:
+forall u u' ex inum s1 s2,
+let p1 := (@lift_L2 AuthenticationOperation _ TD _ (Inode.get_all_block_numbers inum)) in
+let p2 := (@lift_L2 AuthenticationOperation _ TD _ (Inode.get_all_block_numbers inum)) in
+
+refines_related ATC_Refinement (AD_related_states u' ex) s1 s2 ->
+ATC_have_same_structure (ATC_Refinement.(Simulation.Definitions.compile) p1) 
+(ATC_Refinement.(Simulation.Definitions.compile) p2) u s1 s2.
+Proof.
+  Transparent Inode.get_all_block_numbers.
+  unfold Inode.get_all_block_numbers; simpl; intros; cleanup.
+  intuition eauto.
+  unfold refines_related in *; simpl in *.
+  unfold HC_refines in *; simpl in *.
+  unfold TransactionToTransactionalDisk.Definitions.refines in *; simpl in *;
+  cleanup.
+  unfold AD_related_states, FD_related_states,
+  refines_related in *; simpl in *.
+  unfold FileToFileDisk.Definitions.refines,
+  File.files_rep, File.files_inner_rep in *;
+  logic_clean.
+  simpl in *; cleanup.
+  repeat cleanup_pairs.
+  eapply ATC_HSS_inode_get_inode.
+  7: eauto.
+  7: eauto.
+  7: eauto.
+  all: eauto.
+  eapply refines_related_get_first_none.
+  unfold refines_related in *; simpl in *.
+  unfold HC_refines in *; simpl in *.
+  unfold TransactionToTransactionalDisk.Definitions.refines in *; simpl in *;
+  cleanup.
+  unfold AD_related_states, FD_related_states,
+  refines_related in *; simpl in *.
+  unfold FileToFileDisk.Definitions.refines,
+  File.files_rep, File.files_inner_rep in *;
+  simpl in *; cleanup.
+  eexists (_, _), (_, _).
+  intuition eauto.
+  simpl; do 2 eexists; intuition eauto.
+
+  eapply refines_related_get_first_none.
+  unfold refines_related in *; simpl in *.
+  unfold HC_refines in *; simpl in *.
+  unfold TransactionToTransactionalDisk.Definitions.refines in *; simpl in *;
+  cleanup.
+  unfold AD_related_states, FD_related_states,
+  refines_related in *; simpl in *.
+  unfold FileToFileDisk.Definitions.refines,
+  File.files_rep, File.files_inner_rep in *;
+  simpl in *; cleanup.
+  eexists (_, _), (_, _).
+  intuition eauto.
+  simpl; do 2 eexists; intuition eauto.
+
+  destruct r1, r2; simpl; eauto.
+  Opaque Inode.get_all_block_numbers.
+Qed.
+
+Theorem ATC_HSS_inode_get_owner:
+forall u u' ex inum s1 s2,
+let p1 := (@lift_L2 AuthenticationOperation _ TD _ (Inode.get_owner inum )) in
+let p2 := (@lift_L2 AuthenticationOperation _ TD _ (Inode.get_owner inum )) in
+
+refines_related ATC_Refinement (AD_related_states u' ex) s1 s2 ->
+ATC_have_same_structure (ATC_Refinement.(Simulation.Definitions.compile) p1) 
+(ATC_Refinement.(Simulation.Definitions.compile) p2) u s1 s2.
+Proof.
+  Transparent Inode.get_owner.
+  unfold Inode.get_owner; simpl; intros; cleanup.
+  intuition eauto.
+  unfold refines_related in *; simpl in *.
+  unfold HC_refines in *; simpl in *.
+  unfold TransactionToTransactionalDisk.Definitions.refines in *; simpl in *;
+  cleanup.
+  unfold AD_related_states, FD_related_states,
+  refines_related in *; simpl in *.
+  unfold FileToFileDisk.Definitions.refines,
+  File.files_rep, File.files_inner_rep in *;
+  logic_clean.
+  simpl in *; cleanup.
+  repeat cleanup_pairs.
+  eapply ATC_HSS_inode_get_inode.
+  7: eauto.
+  7: eauto.
+  7: eauto.
+  all: eauto.
+  eapply refines_related_get_first_none.
+  unfold refines_related in *; simpl in *.
+  unfold HC_refines in *; simpl in *.
+  unfold TransactionToTransactionalDisk.Definitions.refines in *; simpl in *;
+  cleanup.
+  unfold AD_related_states, FD_related_states,
+  refines_related in *; simpl in *.
+  unfold FileToFileDisk.Definitions.refines,
+  File.files_rep, File.files_inner_rep in *;
+  simpl in *; cleanup.
+  eexists (_, _), (_, _).
+  intuition eauto.
+  simpl; do 2 eexists; intuition eauto.
+
+  eapply refines_related_get_first_none.
+  unfold refines_related in *; simpl in *.
+  unfold HC_refines in *; simpl in *.
+  unfold TransactionToTransactionalDisk.Definitions.refines in *; simpl in *;
+  cleanup.
+  unfold AD_related_states, FD_related_states,
+  refines_related in *; simpl in *.
+  unfold FileToFileDisk.Definitions.refines,
+  File.files_rep, File.files_inner_rep in *;
+  simpl in *; cleanup.
+  eexists (_, _), (_, _).
+  intuition eauto.
+  simpl; do 2 eexists; intuition eauto.
+
+  destruct r1, r2; simpl; eauto.
+  Opaque Inode.get_owner.
+Qed.
+
+Theorem ATC_HSS_read_inner:
+forall u u' ex inum off s1 s2,
+let p1 := (@lift_L2 AuthenticationOperation _ TD _ (File.read_inner off inum)) in
+let p2 := (@lift_L2 AuthenticationOperation _ TD _ (File.read_inner off inum)) in
+
+refines_related ATC_Refinement (AD_related_states u' ex) s1 s2 ->
+ATC_have_same_structure (ATC_Refinement.(Simulation.Definitions.compile) p1) 
+(ATC_Refinement.(Simulation.Definitions.compile) p2) u s1 s2.
+Proof.
+  simpl; intros; cleanup.
+  intuition eauto.
+  eapply ATC_HSS_inode_get_block_number; eauto.
+  unfold refines_related in *; simpl in *.
+  cleanup.
+
+  eapply_fresh ATC_Simulation.ATC_oracle_refines_finished in H0;
+  eapply_fresh ATC_Simulation.ATC_oracle_refines_finished in H1; eauto.
+  cleanup.
+
+  eapply ATC_Simulation.ATC_exec_lift_finished in H0, H1; eauto;
+  try solve [apply TransactionToTransactionalDisk.Refinement.TC_to_TD_core_simulation_finished];
+    cleanup.
+
+  eapply lift2_invert_exec in H0; cleanup.
+  eapply lift2_invert_exec in H1; cleanup.
+  unfold AD_related_states, FD_related_states,
+  refines_related in *; simpl in *.
+  unfold FileToFileDisk.Definitions.refines,
+  File.files_rep, File.files_inner_rep in *;
+  logic_clean.
+  eapply Inode.get_block_number_finished_precise in H9; eauto.
+  eapply Inode.get_block_number_finished_precise in H10; eauto.
+  cleanup.
+  destruct H9, H10; cleanup; try congruence; try lia.
+  unfold HC_refines, TransactionToTransactionalDisk.Definitions.refines in *; simpl in *; logic_clean.
+  unfold TransactionToTransactionalDisk.Definitions.refines,
+  refines_related in *; simpl in *.
+  intuition eauto.
+   eapply ATC_HSS_diskallocator_read; eauto.
+   {
+      repeat cleanup_pairs; simpl in *.
+      eapply SameRetType.all_block_numbers_in_bound in H23, H25; eauto.
+      intuition.
+      eapply Forall_forall in H23; eauto.
+      apply in_seln; eauto.
+      eapply Forall_forall in H25; eauto.
+      apply in_seln; eauto.
+    }
+    {
+      unfold TransactionToTransactionalDisk.Definitions.refines, AD_related_states, FD_related_states,
+      refines_related in *; simpl in *.
+      repeat cleanup_pairs; simpl in *.
+      
+      unfold Transaction.transaction_rep in *;
+      logic_clean; simpl in *.
+      destruct H1, H8, H22, H24; logic_clean; try congruence. 
+      repeat erewrite BlockAllocatorExistence.used_blocks_are_allocated_2.
+      eauto.
+      4: eauto.
+      8: eauto.
+      all: eauto.
+      all: try rewrite <-H16; 
+      try rewrite <- H3; eauto.
+    }
+    {
+      unfold refines_related in *; simpl in *.
+      unfold AD_related_states, FD_related_states,
+      refines_related in *; simpl in *.
+      unfold FileToFileDisk.Definitions.refines,
+      File.files_rep, File.files_inner_rep in *.
+      unfold HC_refines, TransactionToTransactionalDisk.Definitions.refines in *; simpl in *.
+      unfold TransactionToTransactionalDisk.Definitions.refines,
+      refines_related in *; simpl in *.
+      eexists (_, _), (_, _).
+      simpl; intuition eauto.
+      repeat cleanup_pairs.
+      do 2 eexists; intuition eauto.
+    }
+    destruct r1, r2; simpl; eauto.
+    {
+      repeat split_ors; cleanup; try lia.
+      {
+        eapply FileInnerSpecs.inode_exists_then_file_exists in H24; eauto.
+        eapply FileInnerSpecs.inode_missing_then_file_missing in H10; eauto.
+        cleanup.
+        edestruct H11.
+        edestruct H23.
+        intuition; eauto.
+        exfalso; eapply H25; intuition eauto.
+        congruence.
+      }
+      {
+        eapply_fresh FileInnerSpecs.inode_exists_then_file_exists in H10;
+        eapply_fresh FileInnerSpecs.inode_exists_then_file_exists in H24; eauto.
+        cleanup.
+        edestruct H11; cleanup.
+        eapply_fresh H28 in H23; eauto; cleanup.
+        unfold File.file_map_rep in *; logic_clean.
+        eapply H31 in H25;
+        eapply H33 in H23;
+        eauto.
+        unfold File.file_rep in *; cleanup.
+        lia.
+      }
+    }
+    {
+      repeat split_ors; cleanup; try lia.
+      {
+        eapply FileInnerSpecs.inode_exists_then_file_exists in H23; eauto.
+        eapply FileInnerSpecs.inode_missing_then_file_missing in H9; eauto.
+        cleanup.
+        edestruct H11.
+        edestruct H23.
+        intuition; eauto.
+        exfalso; eapply H26; intuition eauto.
+        congruence.
+      }
+      {
+        eapply_fresh FileInnerSpecs.inode_exists_then_file_exists in H9;
+        eapply_fresh FileInnerSpecs.inode_exists_then_file_exists in H23; eauto.
+        cleanup.
+        edestruct H11; cleanup.
+        eapply_fresh H28 in H24; eauto; cleanup.
+        unfold File.file_map_rep in *; logic_clean.
+        eapply H31 in H24;
+        eapply H33 in H25;
+        eauto.
+        unfold File.file_rep in *; cleanup.
+        lia.
+      }
+    }
+    simpl; eauto.
+    Unshelve.
+    all: exact id.
+Qed.
+
+  Theorem ATC_HSS_write_inner:
+  forall u u' ex inum off v1 v2 s1 s2,
+  let p1 := (@lift_L2 AuthenticationOperation _ TD _ (File.write_inner off v1 inum)) in
+  let p2 := (@lift_L2 AuthenticationOperation _ TD _ (File.write_inner off v2 inum)) in
+  
+  refines_related ATC_Refinement (AD_related_states u' ex) s1 s2 ->
+  ATC_have_same_structure (ATC_Refinement.(Simulation.Definitions.compile) p1) 
+  (ATC_Refinement.(Simulation.Definitions.compile) p2) u s1 s2.
+  Proof.
+    simpl; intros; cleanup.
+    intuition eauto.
+    eapply ATC_HSS_inode_get_block_number; eauto.
+    unfold refines_related in *; simpl in *.
+    cleanup.
+
+    eapply_fresh ATC_Simulation.ATC_oracle_refines_finished in H0;
+    eapply_fresh ATC_Simulation.ATC_oracle_refines_finished in H1; eauto.
+    cleanup.
+    eapply ATC_Simulation.ATC_exec_lift_finished in H0, H1; eauto;
+    try solve [apply TransactionToTransactionalDisk.Refinement.TC_to_TD_core_simulation_finished];
+    cleanup.
+
+    eapply lift2_invert_exec in H0; cleanup.
+    eapply lift2_invert_exec in H1; cleanup.
+    unfold AD_related_states, FD_related_states,
+      refines_related in *; simpl in *.
+      unfold FileToFileDisk.Definitions.refines,
+      File.files_rep, File.files_inner_rep in *;
+      logic_clean.
+    eapply Inode.get_block_number_finished in H9; eauto.
+    eapply Inode.get_block_number_finished in H10; eauto.
+    cleanup.
+    destruct H9, H10; cleanup; try congruence; try lia.
+    unfold HC_refines, TransactionToTransactionalDisk.Definitions.refines in *; simpl in *; logic_clean.
+    unfold TransactionToTransactionalDisk.Definitions.refines,
+    refines_related in *; simpl in *.
+    eapply ATC_HSS_diskallocator_write; eauto.
+    {
+      repeat cleanup_pairs; simpl in *.
+      eapply SameRetType.all_block_numbers_in_bound in H29, H31; eauto.
+      intuition.
+      eapply Forall_forall in H29; eauto.
+      apply in_seln; eauto.
+      eapply Forall_forall in H31; eauto.
+      apply in_seln; eauto.
+      eapply File.DiskAllocator.block_allocator_rep_inbounds_eq; eauto.
+      intros; repeat FileInnerSpecs.solve_bounds.
+      eapply File.DiskAllocator.block_allocator_rep_inbounds_eq; eauto.
+      intros; repeat FileInnerSpecs.solve_bounds.
+    }
+    {
+      unfold TransactionToTransactionalDisk.Definitions.refines, AD_related_states, FD_related_states,
+      refines_related in *; simpl in *.
+      repeat cleanup_pairs; simpl in *.
+      
+      unfold Transaction.transaction_rep in *;
+      logic_clean; simpl in *.
+      repeat cleanup_pairs; simpl in *.
+      repeat erewrite BlockAllocatorExistence.used_blocks_are_allocated_2; eauto.
+      eapply File.DiskAllocator.block_allocator_rep_inbounds_eq; eauto.
+      intros; repeat FileInnerSpecs.solve_bounds.
+      eapply File.DiskAllocator.block_allocator_rep_inbounds_eq; eauto.
+      intros; repeat FileInnerSpecs.solve_bounds.
+    }
+    {
+      unfold Transaction.transaction_rep in *;
+      logic_clean; simpl in *.
+      repeat cleanup_pairs; simpl in *.
+      eauto.
+      repeat split_ors; cleanup; try congruence.
+      repeat rewrite map_length in *;
+      destruct s, s0; simpl in *; try lia.
+      intuition eauto.
+    }
+    {
+      unfold Transaction.transaction_rep in *;
+      logic_clean; simpl in *.
+      repeat cleanup_pairs; simpl in *.
+      eauto.
+      repeat split_ors; cleanup; try congruence.
+      repeat rewrite map_length in *;
+      destruct s, s0; simpl in *; try lia.
+      erewrite addr_list_to_blocks_length_eq with (l_b := [File.DiskAllocatorParams.bitmap_addr +
+      S (seln (Inode.block_numbers x11) off 0)]); simpl; eauto.
+      intuition eauto.
+    }
+    {
+      repeat split_ors; cleanup; try lia.
+      {
+        eapply FileInnerSpecs.inode_exists_then_file_exists in H30; eauto.
+        eapply FileInnerSpecs.inode_missing_then_file_missing in H10; eauto.
+        cleanup.
+        edestruct H11.
+        edestruct H29.
+        intuition; eauto.
+        exfalso; eapply H31; intuition eauto.
+        congruence.
+      }
+      {
+        eapply_fresh FileInnerSpecs.inode_exists_then_file_exists in H10;
+        eapply_fresh FileInnerSpecs.inode_exists_then_file_exists in H30; eauto.
+        cleanup.
+        edestruct H11; cleanup.
+        eapply_fresh H34 in H29; eauto; cleanup.
+        unfold File.file_map_rep in *; logic_clean.
+        eapply H37 in H31;
+        eapply H39 in H29;
+        eauto.
+        unfold File.file_rep in *; cleanup.
+        lia.
+      }
+    }
+    {
+      repeat split_ors; cleanup; try lia.
+      {
+        eapply FileInnerSpecs.inode_exists_then_file_exists in H29; eauto.
+        eapply FileInnerSpecs.inode_missing_then_file_missing in H9; eauto.
+        cleanup.
+        edestruct H11.
+        edestruct H29.
+        intuition; eauto.
+        exfalso; eapply H32; intuition eauto.
+        congruence.
+      }
+      {
+        eapply_fresh FileInnerSpecs.inode_exists_then_file_exists in H9;
+        eapply_fresh FileInnerSpecs.inode_exists_then_file_exists in H29; eauto.
+        cleanup.
+        edestruct H11; cleanup.
+        eapply_fresh H34 in H30; eauto; cleanup.
+        unfold File.file_map_rep in *; logic_clean.
+        eapply H37 in H30;
+        eapply H39 in H31;
+        eauto.
+        unfold File.file_rep in *; cleanup.
+        lia.
+      }
+    }
+    simpl; eauto.
+    Unshelve.
+    all: exact id.
+Qed.
+
+Theorem ATC_HSS_change_owner_inner:
+forall u u' ex inum off s1 s2,
+let p1 := (@lift_L2 AuthenticationOperation _ TD _ (File.change_owner_inner off inum)) in
+let p2 := (@lift_L2 AuthenticationOperation _ TD _ (File.change_owner_inner off inum)) in
+
+refines_related ATC_Refinement (AD_related_states u' ex) s1 s2 ->
+ATC_have_same_structure (ATC_Refinement.(Simulation.Definitions.compile) p1) 
+(ATC_Refinement.(Simulation.Definitions.compile) p2) u s1 s2.
+Proof.
+  Transparent Inode.change_owner.
+  unfold File.change_owner_inner, Inode.change_owner; simpl; intros; cleanup.
+  intuition eauto.
+  eapply ATC_HSS_inode_get_block_number; eauto.
+  unfold refines_related in *; simpl in *.
+  cleanup.
+
+  eapply_fresh ATC_Simulation.ATC_oracle_refines_finished in H0;
+  eapply_fresh ATC_Simulation.ATC_oracle_refines_finished in H1; eauto.
+  cleanup.
+  eapply ATC_Simulation.ATC_exec_lift_finished in H0, H1; eauto;
+  try solve [apply TransactionToTransactionalDisk.Refinement.TC_to_TD_core_simulation_finished];
+  cleanup.
+
+  eapply lift2_invert_exec in H0; cleanup.
+  eapply lift2_invert_exec in H1; cleanup.
+  unfold AD_related_states, FD_related_states,
+    refines_related in *; simpl in *.
+    unfold FileToFileDisk.Definitions.refines,
+    File.files_rep, File.files_inner_rep in *;
+    logic_clean.
+  eapply Inode.get_inode_finished_precise in H9; eauto.
+  eapply Inode.get_inode_finished_precise in H10; eauto.
+  cleanup.
+  destruct H9, H10; cleanup; try congruence; try lia.
+  unfold HC_refines, TransactionToTransactionalDisk.Definitions.refines in *; simpl in *; logic_clean.
+  unfold TransactionToTransactionalDisk.Definitions.refines,
+  refines_related in *; simpl in *.
+  eapply ATC_HSS_inode_set_inode. 
+  4: eauto. 
+  4: eauto. 
+  all: eauto.
+  {
+    repeat cleanup_pairs; simpl in *.
+    unfold TransactionToTransactionalDisk.Definitions.refines, AD_related_states, FD_related_states,
+    refines_related in *; simpl in *.
+    repeat cleanup_pairs; simpl in *.
+    
+    unfold Transaction.transaction_rep in *;
+    logic_clean; simpl in *.
+    repeat split_ors; logic_clean; try congruence.
+    repeat rewrite map_length in *.
+    destruct s0, s3; simpl in *.
+    destruct s0, s3; simpl in *; eauto; try lia.
+    intuition eauto.
+  }
+  {
+    unfold TransactionToTransactionalDisk.Definitions.refines, AD_related_states, FD_related_states,
+    refines_related in *; simpl in *.
+    repeat cleanup_pairs; simpl in *.
+    
+    unfold Transaction.transaction_rep in *;
+    logic_clean; simpl in *.
+    repeat split_ors; logic_clean; try congruence.
+    eapply BlockAllocatorExistence.inode_allocations_are_same; eauto.
+    destruct H11.
+    unfold File.file_map_rep in *; logic_clean.
+    eapply BlockAllocatorExistence.addrs_match_exactly_trans; eauto.
+    eapply BlockAllocatorExistence.addrs_match_exactly_sym; eauto.
+    eapply BlockAllocatorExistence.addrs_match_exactly_trans; eauto.
+  }
+  {
+    repeat cleanup_pairs; simpl in *.
+    unfold TransactionToTransactionalDisk.Definitions.refines, AD_related_states, FD_related_states,
+    refines_related in *; simpl in *.
+    repeat cleanup_pairs; simpl in *.
+    
+    unfold Transaction.transaction_rep in *;
+    logic_clean; simpl in *.
+    repeat split_ors; logic_clean; try congruence.
+    repeat rewrite map_length in *.
+    destruct s0, s3; simpl in *.
+    destruct s0, s3; simpl in *; eauto; try lia.
+  }
+  {
+    eapply FileInnerSpecs.inode_exists_then_file_exists in H23; eauto.
+    eapply FileInnerSpecs.inode_missing_then_file_missing in H22; eauto.
+    cleanup.
+    edestruct H11.
+    edestruct H10.
+    intuition; eauto.
+    exfalso; eapply H25; intuition eauto.
+    congruence.
+  }
+  {
+    eapply FileInnerSpecs.inode_exists_then_file_exists in H22; eauto.
+    eapply FileInnerSpecs.inode_missing_then_file_missing in H24; eauto.
+    cleanup.
+    edestruct H11.
+    edestruct H10.
+    intuition; eauto.
+    exfalso; eapply H26; intuition eauto.
+    congruence.
+  }
+  simpl; eauto.
+  Unshelve.
+  all: exact id.
+Qed.
+
+
+Opaque File.DiskAllocator.alloc.
+
+Theorem ATC_HSS_extend_inner:
+  forall u u' ex inum v1 v2 s1 s2 x x0,
+  let p1 := (@lift_L2 AuthenticationOperation _ TD _ (File.extend_inner v1 inum)) in
+  let p2 := (@lift_L2 AuthenticationOperation _ TD _ (File.extend_inner v2 inum)) in
+  
+  @HC_refines _ _ _ Definitions.imp ATCLang _ Definitions.TDCoreRefinement s1 x ->
+  @HC_refines _ _ _ Definitions.imp ATCLang _  Definitions.TDCoreRefinement s2 x0 ->
+  AD_related_states u' ex x x0 ->
+  have_same_structure p1 p2 u x x0 ->
+  inum < Inode.InodeAllocatorParams.num_of_blocks ->
+  ATC_have_same_structure (ATC_Refinement.(Simulation.Definitions.compile) p1) 
+  (ATC_Refinement.(Simulation.Definitions.compile) p2) u s1 s2.
+  Proof.
+    unfold File.extend_inner; intros; cleanup.
+    simpl; intuition eauto.
+
+    eapply ATC_HSS_diskallocator_alloc; eauto.
+    unfold refines_related in *; simpl in *; 
+    unfold HC_refines in *; simpl in *.
+    do 2 eexists; intuition eauto.
+    cleanup.
+
+    unfold refines_related in *; simpl in *; cleanup.
+    eapply_fresh ATC_Simulation.ATC_oracle_refines_finished in H4;
+    eapply_fresh ATC_Simulation.ATC_oracle_refines_finished in H5; eauto.
+    cleanup.
+    eapply_fresh ATC_Simulation.ATC_exec_lift_finished in H4;
+    eapply_fresh ATC_Simulation.ATC_exec_lift_finished in H5; eauto;
+    try solve [apply TransactionToTransactionalDisk.Refinement.TC_to_TD_core_simulation_finished];
+    cleanup.
+
+    eapply_fresh ATC_oracle_refines_impl_eq in H7.
+    4: eauto.
+    4: eauto.
+    all: eauto.
+    2: apply TD_oracle_refines_operation_eq.
+
+    cleanup.
+    eapply_fresh lift2_invert_exec in H9; cleanup.
+    eapply_fresh lift2_invert_exec in H10; cleanup.
+    apply HC_map_ext_eq in H13; subst.
+    eapply_fresh File.DiskAllocator.alloc_finished_oracle_eq in H15; eauto.
+    cleanup.
+    unfold AD_related_states, FD_related_states,
+    refines_related in *; simpl in *.
+    unfold FileToFileDisk.Definitions.refines,
+    File.files_rep, File.files_inner_rep in *;
+    logic_clean.
+    eapply File.DiskAllocator.alloc_finished in H15; eauto.
+    eapply File.DiskAllocator.alloc_finished in H17; eauto.
+    cleanup.
+    destruct H15, H17; cleanup; try congruence; try lia; try solve [intuition congruence].
+    unfold HC_refines, TransactionToTransactionalDisk.Definitions.refines in *; simpl in *; logic_clean.
+    unfold TransactionToTransactionalDisk.Definitions.refines,
+    refines_related in *; simpl in *.
+    repeat cleanup_pairs.
+    eapply disk_allocator_alloc_exact_txn in H4; eauto.
+    eapply disk_allocator_alloc_exact_txn in H5; eauto.
+    repeat split_ors; cleanup; try congruence; simpl in *.
+    eapply ATC_HSS_inode_extend.
+    7: eauto.
+    7: eauto.
+    7: eauto.
+    all: try solve [simpl; eauto].
+    {
+      simpl; cleanup.
+      setoid_rewrite H11;
+      setoid_rewrite H1.
+      simpl in *.
+      destruct (addr_eq_dec Inode.InodeAllocatorParams.bitmap_addr
+      File.DiskAllocatorParams.bitmap_addr); try intuition congruence.
+      destruct (addr_eq_dec Inode.InodeAllocatorParams.bitmap_addr
+      (File.DiskAllocatorParams.bitmap_addr + S x3));
+      destruct (addr_eq_dec Inode.InodeAllocatorParams.bitmap_addr
+      (File.DiskAllocatorParams.bitmap_addr + S x)); try intuition congruence.
+      pose proof inodes_before_data.
+      unfold File.DiskAllocatorParams.bitmap_addr,
+      Inode.InodeAllocatorParams.bitmap_addr in *; lia.
+      pose proof inodes_before_data.
+      unfold File.DiskAllocatorParams.bitmap_addr,
+      Inode.InodeAllocatorParams.bitmap_addr in *; lia.
+
+      clear H15 H17.
+      unfold Transaction.transaction_rep in *;
+      logic_clean; simpl in *.
+      repeat split_ors; logic_clean; try congruence.
+      repeat rewrite map_length in *;
+      destruct s6, s9; simpl in *.
+      destruct s0, s3; simpl in *; try lia.
+      intuition eauto.
+    }
+    {
+      simpl; cleanup.
+      setoid_rewrite H11;
+      setoid_rewrite H1.
+      simpl in *.
+      destruct (addr_eq_dec (Inode.InodeAllocatorParams.bitmap_addr + S inum)
+      File.DiskAllocatorParams.bitmap_addr); try intuition congruence.
+      destruct (addr_eq_dec (Inode.InodeAllocatorParams.bitmap_addr + S inum)
+      (File.DiskAllocatorParams.bitmap_addr + S x3));
+      destruct (addr_eq_dec (Inode.InodeAllocatorParams.bitmap_addr + S inum)
+      (File.DiskAllocatorParams.bitmap_addr + S x)); try intuition congruence.
+      pose proof inodes_before_data.
+      unfold File.DiskAllocatorParams.bitmap_addr,
+      Inode.InodeAllocatorParams.bitmap_addr,
+      Inode.InodeAllocatorParams.num_of_blocks in *; lia.
+      pose proof inodes_before_data.
+      unfold File.DiskAllocatorParams.bitmap_addr,
+      Inode.InodeAllocatorParams.bitmap_addr,
+      Inode.InodeAllocatorParams.num_of_blocks in *; lia.
+
+      clear H15 H17.
+      unfold Transaction.transaction_rep in *;
+      logic_clean; simpl in *.
+      repeat split_ors; logic_clean; try congruence.
+      repeat rewrite map_length in *;
+      destruct s6, s9; simpl in *.
+      destruct s0, s3; simpl in *; try lia.
+      intuition eauto.
+    }
+    {
+      unfold Inode.inode_rep in *; simpl in *;
+      logic_clean.
+      eexists; intuition eauto.
+      eapply Inode.InodeAllocator.block_allocator_rep_inbounds_eq; eauto.
+      intros; repeat FileInnerSpecs.solve_bounds.
+    }
+    {
+      unfold Inode.inode_rep in *; simpl in *;
+      logic_clean.
+      eexists; intuition eauto.
+      eapply Inode.InodeAllocator.block_allocator_rep_inbounds_eq; eauto.
+      intros; repeat FileInnerSpecs.solve_bounds.
+    }
+    {
+      simpl; cleanup.
+      setoid_rewrite H11;
+      setoid_rewrite H1.
+      simpl in *.
+      clear H15 H17.
+      unfold Transaction.transaction_rep in *;
+      logic_clean; simpl in *.
+      repeat split_ors; logic_clean; try congruence.
+      repeat rewrite map_length in *;
+      destruct s6, s9; simpl in *.
+      destruct s0, s3; simpl in *; try lia.
+    }
+    Unshelve.
+    all: eauto; exact id.
+Qed.
+
+Opaque Transaction.commit.
+Theorem ATC_HSS_create:
+  forall u u' u'' ex s1 s2 x x0,
+  let p1 := (File.create u'') in
+  let p2 := (File.create u'') in
+  @HC_refines _ _ _ Definitions.imp ATCLang _ Definitions.TDCoreRefinement s1 x ->
+  @HC_refines _ _ _ Definitions.imp ATCLang _  Definitions.TDCoreRefinement s2 x0 ->
+  AD_related_states u' ex x x0 ->
+  have_same_structure p1 p2 u x x0 ->
+  ATC_have_same_structure (ATC_Refinement.(Simulation.Definitions.compile) p1) 
+  (ATC_Refinement.(Simulation.Definitions.compile) p2) u s1 s2.
+  Proof.
+    unfold File.create; intros; cleanup.
+    simpl; intuition eauto.
+    unfold refines_related in *; simpl in *.
+    unfold HC_refines in *; simpl in *.
+    unfold TransactionToTransactionalDisk.Definitions.refines in *.
+    cleanup.
+
+    eapply ATC_HSS_inodeallocator_alloc; eauto.
+    unfold refines_related in *; simpl in *; 
+    unfold HC_refines in *; simpl in *.
+    do 2 eexists; intuition eauto.
+    cleanup.
+
+    unfold refines_related in *; simpl in *; cleanup.
+    eapply_fresh ATC_Simulation.ATC_oracle_refines_finished in H3;
+    eapply_fresh ATC_Simulation.ATC_oracle_refines_finished in H4; eauto.
+    cleanup.
+    eapply_fresh ATC_Simulation.ATC_exec_lift_finished in H3;
+    eapply_fresh ATC_Simulation.ATC_exec_lift_finished in H4; eauto;
+    try solve [apply TransactionToTransactionalDisk.Refinement.TC_to_TD_core_simulation_finished];
+    cleanup.
+
+    eapply_fresh ATC_oracle_refines_impl_eq in H6.
+    4: eauto.
+    4: eauto.
+    all: eauto.
+    2: apply TD_oracle_refines_operation_eq.
+
+    cleanup.
+    eapply_fresh H7 in H9; eauto.
+
+    eapply_fresh lift2_invert_exec in H8; cleanup_no_match.
+    eapply_fresh lift2_invert_exec in H9; cleanup_no_match.
+    unfold AD_related_states, FD_related_states,
+    refines_related in *; simpl in *.
+    unfold FileToFileDisk.Definitions.refines,
+    File.files_rep, File.files_inner_rep in *;
+    logic_clean.
+    eapply_fresh Inode.alloc_finished in H14; eauto.
+    eapply_fresh Inode.alloc_finished in H16; eauto.
+    cleanup_no_match.
+    destruct H26, H29; cleanup; simpl in *; try congruence; try lia;
+    try solve [intuition congruence].
+    simpl; intuition eauto; try congruence.
+    unfold HC_refines in *; simpl in *.
+    unfold TransactionToTransactionalDisk.Definitions.refines in *; logic_clean.
+    eapply inode_allocator_alloc_exact_txn in H3, H4; eauto.
+    repeat split_ors; try logic_clean; try congruence.
+    eapply ATC_HSS_transaction_commit.
+    {
+      cleanup.
+      setoid_rewrite H50;
+      setoid_rewrite H53.
+      simpl.
+      clear H46 H47.
+      unfold Transaction.transaction_rep in *;
+      logic_clean; simpl in *.
+      repeat split_ors; logic_clean; try congruence.
+      repeat cleanup_pairs.
+      repeat rewrite map_length in *;
+      destruct s1, s4; simpl in *; try lia.
+      destruct (addr_dec Inode.InodeAllocatorParams.bitmap_addr
+      (Inode.InodeAllocatorParams.bitmap_addr + S x11));
+      destruct (addr_dec Inode.InodeAllocatorParams.bitmap_addr
+      (Inode.InodeAllocatorParams.bitmap_addr + S x12)); try lia.
+      simpl; eauto.
+    }
+    {
+      cleanup.
+      setoid_rewrite H50;
+      setoid_rewrite H53.
+      simpl.
+      clear H46 H47.
+      unfold Transaction.transaction_rep in *;
+      logic_clean; simpl in *.
+      repeat split_ors; logic_clean; try congruence.
+      repeat cleanup_pairs.
+      repeat rewrite map_length in *;
+      destruct s1, s4; simpl in *; try lia.
+      pose proof inodes_fit_in_disk.
+      unfold Inode.InodeAllocatorParams.bitmap_addr,
+      Inode.InodeAllocatorParams.num_of_blocks in *;
+      intuition; repeat constructor.
+    }
+    Unshelve.
+    all: eauto; constructor.
+Qed.
+
+
+Theorem ATC_HSS_free_all_blocks:
+  forall u l1 l2 s1 s2 td1 td2 dh1 dh2,
+  let p1 := (@lift_L2 AuthenticationOperation _ TD _ (File.free_all_blocks l1)) in
+  let p2 := (@lift_L2 AuthenticationOperation _ TD _ (File.free_all_blocks l2)) in
+  Forall2 (fun a1 a2 => a1 < File.DiskAllocatorParams.num_of_blocks <->
+  a2 < File.DiskAllocatorParams.num_of_blocks) l1 l2 ->
+  Forall (fun a1 => test_bit a1 (value_to_bits (fst (snd (snd td1)) File.DiskAllocatorParams.bitmap_addr)) = true) l1 ->
+  Forall (fun a1 => test_bit a1 (value_to_bits (fst (snd (snd td2)) File.DiskAllocatorParams.bitmap_addr)) = true) l2 ->
+  NoDup l1 ->
+  NoDup l2 ->
+  (Transaction.get_first (fst (snd s1)) File.DiskAllocatorParams.bitmap_addr =
+  None <->
+  Transaction.get_first (fst (snd s2)) File.DiskAllocatorParams.bitmap_addr =
+  None) ->
+  @HC_refines _ _ _ Definitions.imp ATCLang AD Definitions.TDCoreRefinement s1 td1 ->
+  @HC_refines _ _ _ Definitions.imp ATCLang AD  Definitions.TDCoreRefinement s2 td2 ->
+  File.DiskAllocator.block_allocator_rep dh1 (fst (snd (snd td1))) ->
+  File.DiskAllocator.block_allocator_rep dh2 (fst (snd (snd td2))) ->
+  length (fst (snd s1)) = length (fst (snd s2)) ->
+  have_same_structure p1 p2 u td1 td2 ->
+  ATC_have_same_structure (ATC_Refinement.(Simulation.Definitions.compile) p1) 
+  (ATC_Refinement.(Simulation.Definitions.compile) p2) u s1 s2.
+  Proof.
+  induction l1; destruct l2; simpl in *; intros; eauto; 
+  inversion H; inversion H0; 
+  inversion H1; inversion H2; 
+  inversion H3; cleanup; try lia.
+  intuition eauto.
+  eapply ATC_HSS_diskallocator_free; eauto.
+  intuition eauto.
+  intuition eauto.
+
+  unfold HC_refines in *; cleanup; eauto.
+  unfold HC_refines in *; cleanup; eauto.
+
+  unfold refines_related in *; simpl in *; cleanup.
+  eapply_fresh ATC_Simulation.ATC_oracle_refines_finished in H13;
+  eapply_fresh ATC_Simulation.ATC_oracle_refines_finished in H14; eauto.
+  cleanup.
+  eapply_fresh ATC_Simulation.ATC_exec_lift_finished in H13;
+  eapply_fresh ATC_Simulation.ATC_exec_lift_finished in H14; eauto;
+  try solve [apply TransactionToTransactionalDisk.Refinement.TC_to_TD_core_simulation_finished];
+  cleanup.
+
+  eapply_fresh ATC_oracle_refines_impl_eq in H34.
+  4: eauto.
+  4: eauto.
+  all: eauto.
+  2: apply TD_oracle_refines_operation_eq.
+  cleanup.
+  eapply_fresh H35 in H21; eauto.
+  
+  eapply_fresh lift2_invert_exec in H18; logic_clean.
+  eapply_fresh lift2_invert_exec in H21; logic_clean.
+  unfold HC_refines, TransactionToTransactionalDisk.Definitions.refines in *; simpl in *; logic_clean.
+  eapply File.DiskAllocator.free_finished in H30; eauto.
+  eapply File.DiskAllocator.free_finished in H37; eauto.
+  eapply diskallocator_free_exact_txn in H13, H14; eauto.
+  cleanup_no_match; repeat split_ors; cleanup_no_match; simpl in *; try tauto.
+  unfold HC_refines, TransactionToTransactionalDisk.Definitions.refines in *; simpl in *; logic_clean.
+  unfold TransactionToTransactionalDisk.Definitions.refines,
+  refines_related in *; simpl in *.
+  repeat cleanup_pairs.
+
+  eapply IHl1; simpl; eauto.
+  all: simpl; eauto.
+  {
+    eapply Forall_forall; intros.
+    unfold File.DiskAllocator.block_allocator_rep in *; simpl in *; logic_clean.
+    destruct  (Compare_dec.lt_dec x1 (length x5)).
+    {
+      eapply File.DiskAllocator.valid_bits_extract in H22; eauto.
+      eapply File.DiskAllocator.valid_bits_extract with (n := x1)in H45; eauto.
+      logic_clean.
+      repeat split_ors; cleanup; eauto.
+      eapply Forall_forall in H20; eauto; try congruence.
+      rewrite delete_ne in H50; eauto; try congruence.
+      all: lia.
+    }
+    {
+      destruct (H47 x1).
+      lia.
+      eapply Forall_forall in H20; eauto; try congruence.
+    }
+  }
+  {
+    eapply Forall_forall; intros.
+    unfold File.DiskAllocator.block_allocator_rep in *; simpl in *; logic_clean.
+    destruct  (Compare_dec.lt_dec x1 (length x7)).
+    {
+      eapply File.DiskAllocator.valid_bits_extract in H30; eauto.
+      eapply File.DiskAllocator.valid_bits_extract with (n := x1) in H41; eauto.
+      logic_clean.
+      repeat split_ors; cleanup; eauto.
+      eapply Forall_forall in H24; eauto; try congruence.
+      rewrite delete_ne in H50; eauto; try congruence.
+      all: lia.
+    }
+    {
+      destruct (H44 x1).
+      lia.
+      eapply Forall_forall in H24; eauto; try congruence.
+    }
+  }
+  {
+    destruct (addr_eq_dec File.DiskAllocatorParams.bitmap_addr
+    File.DiskAllocatorParams.bitmap_addr); try lia; intuition congruence.
+  }
+  {
+    destruct l1; simpl in *; eauto.
+  }
+  {
+    destruct l2; simpl in *; eauto.
+  }
+  Unshelve.
+  all: try exact id; constructor.
+  Qed.
+
+
+
+Theorem ATC_HSS_delete_inner:
+  forall u u' ex inum s1 s2 x x0,
+  let p1 := (@lift_L2 AuthenticationOperation _ TD _ (File.delete_inner inum)) in
+  let p2 := (@lift_L2 AuthenticationOperation _ TD _ (File.delete_inner inum)) in
+  
+  @HC_refines _ _ _ Definitions.imp ATCLang _ Definitions.TDCoreRefinement s1 x ->
+  @HC_refines _ _ _ Definitions.imp ATCLang _  Definitions.TDCoreRefinement s2 x0 ->
+  AD_related_states u' ex x x0 ->
+  have_same_structure p1 p2 u x x0 ->
+  ATC_have_same_structure (ATC_Refinement.(Simulation.Definitions.compile) p1) 
+  (ATC_Refinement.(Simulation.Definitions.compile) p2) u s1 s2.
+  Proof.
+    unfold File.delete_inner; intros; cleanup.
+    simpl; intuition eauto.
+    unfold refines_related in *; simpl in *.
+    unfold HC_refines in *; simpl in *.
+    unfold TransactionToTransactionalDisk.Definitions.refines in *.
+    cleanup.
+
+    eapply ATC_HSS_inode_get_all_block_numbers; eauto.
+    unfold refines_related in *; simpl in *; 
+    unfold HC_refines in *; simpl in *.
+    do 2 eexists; intuition eauto.
+    
+    unfold refines_related in *; simpl in *; cleanup.
+    eapply_fresh ATC_Simulation.ATC_oracle_refines_finished in H3;
+    eapply_fresh ATC_Simulation.ATC_oracle_refines_finished in H4; eauto.
+    cleanup.
+    eapply_fresh ATC_Simulation.ATC_exec_lift_finished in H3;
+    eapply_fresh ATC_Simulation.ATC_exec_lift_finished in H4; eauto;
+    try solve [apply TransactionToTransactionalDisk.Refinement.TC_to_TD_core_simulation_finished];
+    cleanup.
+
+    eapply_fresh ATC_oracle_refines_impl_eq in H6.
+    4: eauto.
+    4: eauto.
+    all: eauto.
+    2: apply TD_oracle_refines_operation_eq.
+
+    cleanup.
+    eapply_fresh H7 in H9; eauto.
+
+    eapply_fresh lift2_invert_exec in H8; cleanup.
+    eapply_fresh lift2_invert_exec in H9; cleanup.
+    unfold AD_related_states, FD_related_states,
+    refines_related in *; simpl in *.
+    unfold FileToFileDisk.Definitions.refines,
+    File.files_rep, File.files_inner_rep in *;
+    logic_clean.
+    eapply Inode.get_all_block_numbers_finished_precise in H14; eauto.
+    eapply Inode.get_all_block_numbers_finished_precise in H16; eauto.
+    cleanup.
+    destruct H14, H16; simpl in *; cleanup; try congruence; try lia.
+    intuition eauto.
+
+    eapply ATC_HSS_free_all_blocks.
+    7: eauto.
+    7: eauto.
+    all: try solve [simpl; eauto].
+    {
+      eapply forall_forall2.
+      eapply Forall_forall; intros.
+      destruct x13.
+      simpl; intuition.
+      eapply in_combine_r in H14.
+      eapply SameRetType.all_block_numbers_in_bound in H33; eauto.
+      eapply Forall_forall in H33; eauto.
+      apply in_combine_l in H14.
+      eapply SameRetType.all_block_numbers_in_bound in H17; eauto.
+      eapply Forall_forall in H17; eauto.
+
+      eapply_fresh FileInnerSpecs.inode_exists_then_file_exists in H17;
+      eapply_fresh FileInnerSpecs.inode_exists_then_file_exists in H33; eauto.
+     logic_clean.
+      edestruct H22; logic_clean.
+      eapply_fresh H36 in H16; eauto; logic_clean.
+
+      unfold File.file_map_rep in *; logic_clean.
+      eapply H41 in H17;
+      eapply H39 in H33;
+      eauto.
+      unfold File.file_rep in *; logic_clean.
+      setoid_rewrite <- H43;
+      setoid_rewrite <- H45; lia.
+    }
+    {
+      eapply Forall_forall; intros.
+      eapply in_seln_exists in H14; cleanup.
+      unfold HC_refines in *; simpl in *; cleanup; eauto.
+      repeat cleanup_pairs.
+      rewrite <- H16.
+      eapply BlockAllocatorExistence.used_blocks_are_allocated_2; eauto.
+    }
+    {
+      eapply Forall_forall; intros.
+      eapply in_seln_exists in H14; cleanup.
+      unfold HC_refines in *; simpl in *; cleanup; eauto.
+      repeat cleanup_pairs.
+      rewrite <- H16.
+      eapply BlockAllocatorExistence.used_blocks_are_allocated_2; eauto.
+    }
+    {
+      unfold Inode.inode_rep, Inode.inode_map_rep,
+      Inode.inode_map_valid  in *;
+      logic_clean.
+      eapply H36 in H17.
+      unfold Inode.inode_valid in *; logic_clean; eauto.
+    }
+    {
+      unfold Inode.inode_rep, Inode.inode_map_rep,
+      Inode.inode_map_valid  in *;
+      logic_clean.
+      eapply H24 in H33.
+      unfold Inode.inode_valid in *; logic_clean; eauto.
+    }
+    { 
+      unfold HC_refines in *; simpl in *; cleanup; eauto.
+      unfold TransactionToTransactionalDisk.Definitions.refines, AD_related_states, FD_related_states,
+      refines_related in *; simpl in *.
+      repeat cleanup_pairs; simpl in *.
+      
+      unfold Transaction.transaction_rep in *;
+      logic_clean; simpl in *.
+      repeat split_ors; logic_clean; try congruence.
+      repeat rewrite map_length in *; destruct s0, s5; simpl in *.
+      destruct s0, s3; simpl in *; try lia.
+      intuition eauto.
+    }
+    {
+      repeat cleanup_pairs; eauto. 
+    }
+    {
+      repeat cleanup_pairs; eauto. 
+    }
+    { 
+      unfold HC_refines in *; simpl in *; cleanup; eauto.
+      unfold TransactionToTransactionalDisk.Definitions.refines, AD_related_states, FD_related_states,
+      refines_related in *; simpl in *.
+      repeat cleanup_pairs; simpl in *.
+      
+      unfold Transaction.transaction_rep in *;
+      logic_clean; simpl in *.
+      repeat split_ors; logic_clean; try congruence.
+      repeat rewrite map_length in *; destruct s0, s5; simpl in *.
+      destruct s0, s3; simpl in *; try lia.
+    }
+    {
+      unfold refines_related in *; simpl in *; cleanup.
+      eapply_fresh ATC_Simulation.ATC_oracle_refines_finished in H14;
+      eapply_fresh ATC_Simulation.ATC_oracle_refines_finished in H16; eauto.
+      cleanup.
+      eapply_fresh ATC_Simulation.ATC_exec_lift_finished in H14;
+      eapply_fresh ATC_Simulation.ATC_exec_lift_finished in H16; eauto;
+      try solve [apply TransactionToTransactionalDisk.Refinement.TC_to_TD_core_simulation_finished];
+      cleanup.
+
+      eapply_fresh ATC_oracle_refines_impl_eq in H19. 
+      4: eauto.
+      4: eauto.
+      all: eauto.
+      2: apply TD_oracle_refines_operation_eq.
+
+      cleanup.
+      eapply_fresh H20 in H36; eauto.
+
+      eapply_fresh lift2_invert_exec in H36; cleanup_no_match.
+      eapply_fresh lift2_invert_exec in H37; cleanup_no_match.
+      repeat cleanup_pairs; simpl in *.
+      eapply FileInnerSpecs.free_all_blocks_finished in H42; eauto.
+      eapply FileInnerSpecs.free_all_blocks_finished in H44; eauto.
+      cleanup_no_match.
+      destruct H1, H13; simpl in *; cleanup; try congruence; try lia; simpl in *; eauto.
+      Transparent Inode.free.
+      unfold Inode.free, Inode.InodeAllocator.free  in *; simpl in *; 
+      cleanup; try tauto.
+      unfold Inode.free, Inode.InodeAllocator.free  in *; simpl in *; 
+      cleanup; try tauto.
+      Opaque Inode.free.
+
+      unfold HC_refines  in *; simpl in *; cleanup.
+      eapply ATC_HSS_inodeallocator_free. 
+      4: eauto.
+      4: eauto.
+      all: eauto.
+      intuition eauto.
+      {
+        eapply BlockAllocatorExistence.inode_allocations_are_same; eauto.
+        repeat cleanup_pairs.
+        unfold Inode.inode_rep in *; logic_clean.
+        eexists; split.
+        eapply Inode.InodeAllocator.block_allocator_rep_inbounds_eq.
+        apply b.
+        intros; FileInnerSpecs.solve_bounds.
+        eauto.
+
+        repeat cleanup_pairs.
+        unfold Inode.inode_rep in *; logic_clean.
+        eexists; split.
+        eapply Inode.InodeAllocator.block_allocator_rep_inbounds_eq.
+        apply b0.
+        intros; FileInnerSpecs.solve_bounds.
+        eauto.
+        
+        destruct H22.
+        unfold File.file_map_rep in *; logic_clean.
+        eapply BlockAllocatorExistence.addrs_match_exactly_trans; eauto.
+        eapply BlockAllocatorExistence.addrs_match_exactly_sym; eauto.
+        eapply BlockAllocatorExistence.addrs_match_exactly_trans; eauto.
+      }
+      {
+      unfold TransactionToTransactionalDisk.Definitions.refines, AD_related_states, FD_related_states,
+      refines_related in *; simpl in *.
+      repeat cleanup_pairs; simpl in *.
+      
+      eapply free_all_blocks_exact_txn in H14, H16; eauto.
+      repeat split_ors; cleanup; try congruence.
+      simpl in *; cleanup.
+
+      Lemma get_first_none_not_in_rev:
+      forall (l : list (addr * value)) (a : addr),
+      ~ In a (map fst l) -> Transaction.get_first l a = None.
+      Proof.
+        induction l; simpl in *; eauto.
+        intuition; simpl in *.
+        destruct (addr_eq_dec a a0); eauto; lia.
+      Qed.
+      repeat rewrite get_first_none_not_in_rev; eauto.
+      intuition.
+      rewrite map_app; intros Hin.
+      apply in_app_iff in Hin; split_ors.
+      rewrite H14 in H.
+      apply repeat_spec in H.
+      pose proof inodes_before_data.
+      unfold Inode.InodeAllocatorParams.bitmap_addr,
+      File.DiskAllocatorParams.bitmap_addr in *; lia.
+      
+      clear H13 H32 H41 H43.
+      unfold Transaction.transaction_rep in *;
+      logic_clean; simpl in *.
+      repeat split_ors; logic_clean; try congruence.
+      repeat rewrite map_length in *.
+      destruct s0;  simpl in *.
+      destruct s0; simpl in *; try lia.
+
+
+      rewrite map_app; intros Hin.
+      apply in_app_iff in Hin; split_ors.
+      rewrite H48 in H.
+      apply repeat_spec in H.
+      pose proof inodes_before_data.
+      unfold Inode.InodeAllocatorParams.bitmap_addr,
+      File.DiskAllocatorParams.bitmap_addr in *; lia.
+      
+      clear H13 H32 H41 H43.
+      unfold Transaction.transaction_rep in *;
+      logic_clean; simpl in *.
+      repeat split_ors; logic_clean; try congruence.
+      repeat rewrite map_length in *.
+      destruct s5;  simpl in *.
+      destruct s3; simpl in *; try lia.
+      }
+      {
+      unfold TransactionToTransactionalDisk.Definitions.refines, AD_related_states, FD_related_states,
+      refines_related in *; simpl in *.
+      repeat cleanup_pairs; simpl in *.
+      
+      eapply free_all_blocks_exact_txn in H14, H16; eauto.
+      repeat split_ors; cleanup; try congruence.
+      simpl in *; cleanup.
+      repeat rewrite app_length.
+      
+      clear H13 H32 H41 H43.
+      unfold Transaction.transaction_rep in *;
+      logic_clean; simpl in *.
+      repeat split_ors; logic_clean; try congruence.
+      repeat rewrite map_length in *.
+      destruct s0, s5;  simpl in *.
+      destruct s0, s5; simpl in *; try lia.
+
+
+      eapply_fresh FileInnerSpecs.inode_exists_then_file_exists in H17;
+        eapply_fresh FileInnerSpecs.inode_exists_then_file_exists in H33; eauto.
+       logic_clean.
+        edestruct H22; logic_clean.
+        eapply_fresh H67 in H64; eauto; logic_clean.
+
+        unfold File.file_map_rep in *; logic_clean.
+        eapply H72 in H17;
+        eapply H70 in H33;
+        eauto.
+        unfold File.file_rep in *; logic_clean.
+        rewrite H11, H47. 
+        setoid_rewrite <- H74;
+        setoid_rewrite <- H76; lia.
+      }
+    }
+    Unshelve.
+    all: eauto; constructor.
+    Qed.
+
+Theorem ATC_HSS_auth_then_exec:
+  forall u u' T (p1 p2 : addr -> @prog _  TD (option T)) ex inum s1 s2 x x0,
+  let px := (fun inum => @lift_L2 AuthenticationOperation _ TD _ (p1 inum)) in
+  let py := (fun inum => @lift_L2 AuthenticationOperation _ TD _ (p2 inum)) in
+
+  (forall s1 s2 x x0,
+  @HC_refines _ _ _ Definitions.imp ATCLang _ Definitions.TDCoreRefinement s1 x ->
+  @HC_refines _ _ _ Definitions.imp ATCLang _  Definitions.TDCoreRefinement s2 x0 ->
+  AD_related_states u' ex x x0 ->
+  have_same_structure (px inum) (py inum) u x x0 ->
+  inum < Inode.InodeAllocatorParams.num_of_blocks ->
+  ATC_have_same_structure (ATC_Refinement.(Simulation.Definitions.compile) (px inum)) 
+  (ATC_Refinement.(Simulation.Definitions.compile) (py inum)) u s1 s2) ->
+
+  
+  (forall s1 s2 o s1' s2' r1 r2, 
+  refines_related ATC_Refinement (AD_related_states u' ex) s1 s2 ->
+  exec ATCLang u o s1 (ATC_Refinement.(Simulation.Definitions.compile) (px inum)) (Finished s1' (Some r1)) ->
+  exec ATCLang u o s2 (ATC_Refinement.(Simulation.Definitions.compile) (py inum)) (Finished s2' (Some r2)) ->
+  inum < Inode.InodeAllocatorParams.num_of_blocks ->
+  length (dedup_last addr_dec (rev (map fst (fst (snd s1'))))) =
+  length (dedup_last addr_dec (rev (map fst (fst (snd s2'))))) /\
+  (Forall (fun a : nat => a < data_length) (map fst (fst (snd s1'))) <->
+  Forall (fun a : nat => a < data_length) (map fst (fst (snd s2'))))) ->
+
+
+  @HC_refines _ _ _ Definitions.imp ATCLang _ Definitions.TDCoreRefinement s1 x ->
+  @HC_refines _ _ _ Definitions.imp ATCLang _  Definitions.TDCoreRefinement s2 x0 ->
+  AD_related_states u' ex x x0 ->
+  have_same_structure (File.auth_then_exec inum p1) (File.auth_then_exec inum p2) u x x0 ->
+
+  ATC_have_same_structure (ATC_Refinement.(Simulation.Definitions.compile) (File.auth_then_exec inum p1)) 
+  (ATC_Refinement.(Simulation.Definitions.compile) (File.auth_then_exec inum p2)) u s1 s2.
+  Proof.
+    unfold File.auth_then_exec; simpl; intros.
+    intuition eauto.
+    eapply ATC_HSS_inode_get_owner; eauto.
+    unfold refines_related in *; simpl in *; cleanup.
+    do 2 eexists; intuition eauto.
+
+    unfold refines_related in *; simpl in *; cleanup.
+    eapply_fresh ATC_Simulation.ATC_oracle_refines_finished in H7;
+    eapply_fresh ATC_Simulation.ATC_oracle_refines_finished in H9; eauto.
+    cleanup.
+    eapply_fresh ATC_Simulation.ATC_exec_lift_finished in H7;
+    eapply_fresh ATC_Simulation.ATC_exec_lift_finished in H9; eauto;
+    try solve [apply TransactionToTransactionalDisk.Refinement.TC_to_TD_core_simulation_finished];
+    cleanup.
+
+    eapply_fresh ATC_oracle_refines_impl_eq in H6.
+    4: eauto.
+    4: eauto.
+    all: eauto.
+    2: apply TD_oracle_refines_operation_eq.
+    cleanup.
+
+    eapply_fresh lift2_invert_exec in H10; cleanup.
+    eapply_fresh lift2_invert_exec in H11; cleanup.
+    eapply H8 in H10; eauto.
+
+    unfold AD_related_states, FD_related_states,
+    refines_related in *; simpl in *.
+    unfold FileToFileDisk.Definitions.refines,
+    File.files_rep, File.files_inner_rep in *;
+    logic_clean.
+    eapply Inode.get_owner_finished_precise in H16; eauto.
+    eapply Inode.get_owner_finished_precise in H18; eauto.
+    cleanup_no_match.
+    destruct H16, H18; cleanup; simpl in *; 
+    cleanup; try tauto; try congruence; try lia.
+    {
+      unfold HC_refines, TransactionToTransactionalDisk.Definitions.refines in *; simpl in *; logic_clean.
+      unfold TransactionToTransactionalDisk.Definitions.refines,
+      refines_related in *; simpl in *.
+      intuition eauto.
+      assert (
+        exists o s1' s2' , exec AD u o x4
+      (Op (HorizontalComposition AuthenticationOperation
+            (TransactionalDiskLayer.TDCore data_length))
+         ( @P1 AuthenticationOperation _ _ (Auth (Inode.owner x11)) )) (Finished s1' r1) /\
+         exec AD u o x3
+      (Op (HorizontalComposition AuthenticationOperation
+              (TransactionalDiskLayer.TDCore data_length))
+              ( @P1 AuthenticationOperation _ _ (Auth (Inode.owner x12)) )) (Finished s2' r2)). {
+          repeat invert_exec; try congruence;
+          do 3 eexists; split; repeat econstructor; eauto.
+         }
+      logic_clean.
+      eapply_fresh H33 in H38; eauto.
+      repeat invert_exec_no_match;  cleanup;
+      simpl in *; cleanup; eauto; try tauto; try congruence.
+      assert (A: inum < Inode.InodeAllocatorParams.num_of_blocks). {
+        destruct (Compare_dec.lt_dec inum Inode.InodeAllocatorParams.num_of_blocks); eauto.
+          unfold Inode.inode_rep, Inode.inode_map_rep, 
+          Inode.InodeAllocator.block_allocator_rep in *; logic_clean.
+          edestruct (H44 inum); try lia.
+          rewrite H26, H50 in H32.
+          simpl in *;  congruence.
+      }
+      {
+        simpl in *; intuition eauto.
+        {
+          eapply H. 
+          4: eauto. 
+          all: simpl in *; eauto.
+          all: repeat cleanup_pairs; simpl in *; eauto.
+          do 2 eexists; intuition eauto.
+        }
+
+        eapply_fresh ATC_Simulation.ATC_oracle_refines_finished in H17.
+        eapply_fresh ATC_Simulation.ATC_oracle_refines_finished in H38; eauto.
+        cleanup.
+        eapply_fresh ATC_Simulation.ATC_exec_lift_finished in H17; eauto.
+        eapply_fresh ATC_Simulation.ATC_exec_lift_finished in H38; eauto;
+        try solve [apply TransactionToTransactionalDisk.Refinement.TC_to_TD_core_simulation_finished];
+        cleanup.
+        all: try solve [apply TransactionToTransactionalDisk.Refinement.TC_to_TD_core_simulation_finished].
+
+        eapply_fresh ATC_oracle_refines_impl_eq in H39.
+        6: eauto.
+        6: eauto.
+        all: eauto.
+        4: apply TD_oracle_refines_operation_eq.
+        cleanup.
+
+        eapply_fresh lift2_invert_exec in e; cleanup.
+        eapply_fresh lift2_invert_exec in H44; cleanup.
+        eapply H40 in e; eauto.
+        cleanup; simpl in *; cleanup; eauto; try tauto.
+        intuition eauto.
+
+        edestruct H0; eauto.
+        eexists (_, _), (_, _); intuition eauto.
+        do 2 eexists; simpl; intuition eauto.
+        repeat cleanup_pairs; simpl; eauto.
+        repeat cleanup_pairs; simpl; eauto.
+
+        eapply ATC_HSS_transaction_commit; eauto.
+        all: simpl; unfold HC_refines  in *; simpl in *;
+        unfold TransactionToTransactionalDisk.Definitions.refines in *; simpl in *; cleanup; eauto.
+      }
+      {
+        erewrite <- SameRetType.inode_owners_are_same_3 in H43.
+        exfalso; eauto.
+        6: eauto.
+        6: eauto.
+        3: eauto.
+        all: eauto.
+        eapply same_for_user_except_symmetry; eauto.
+      }
+      {
+        erewrite <- SameRetType.inode_owners_are_same_3 in H47.
+        exfalso; eauto.
+        6: eauto.
+        6: eauto.
+        3: eauto.
+        all: eauto.
+      }
+    }
+    Unshelve.
+    all: eauto; constructor.
+  Qed.
